src/SoftBound/sb_ds_trans_correct.v
@@ -19,290 +19,148 @@ Require Import Metatheory.
 Require Import Znumtheory.
 Require Import sb_ds_def.
 Require Import sb_ds_trans.
+Require Import sb_ds_sim.
+Require Import ssa_wf.
 
 Import SB_ds_pass.
 
-(* Simulation *)
-
-Definition meminj_no_overlap (f: meminj) (m: mem) : Prop :=
-  forall b1 b1' delta1 b2 b2' delta2,
-  b1 <> b2 ->
-  f b1 = Some (b1', delta1) ->
-  f b2 = Some (b2', delta2) ->
-  b1' <> b2'.
-
-Lemma meminj_no_overlap__implies : forall f m,
-  meminj_no_overlap f m -> Mem.meminj_no_overlap f m.
-Proof.
-  intros f m J.
-  unfold meminj_no_overlap in J.
-  unfold Mem.meminj_no_overlap.
-  eauto.
-Qed.
-
-Record wf_sb_mi maxb mi Mem1 Mem2 := mk_wf_sb_mi {
-  Hno_overlap : meminj_no_overlap mi Mem1;
-  Hnull : mi Mem.nullptr = Some (Mem.nullptr, 0);
-  Hmap1 : forall b, b >= Mem.nextblock Mem1 -> mi b = None;
-  Hmap2 : forall b1 b2 delta2, 
-    mi b1 = Some (b2, delta2) -> b2 < Mem.nextblock Mem2;
-  mi_freeblocks: forall b, ~(Mem.valid_block Mem1 b) -> mi b = None;
-  mi_mappedblocks: forall b b' delta, 
-    mi b = Some(b', delta) -> Mem.valid_block Mem2 b';
-  mi_range_block: forall b b' delta, 
-    mi b = Some(b', delta) -> delta = 0;
-  mi_bounds: forall b b' delta, 
-    mi b = Some(b', delta) -> Mem.bounds Mem1 b = Mem.bounds Mem2 b';
-  mi_globals : forall b, b <= maxb -> mi b = Some (b, 0)
-  }.
-
-Definition gv_inject (mi: Values.meminj) (gv gv':GenericValue) : Prop :=
-let '(vals,mks) := List.split gv in 
-let '(vals',mks') := List.split gv' in 
-val_list_inject mi vals vals' /\ mks = mks'.
-
-Definition reg_simulation (mi:Values.meminj) TD gl (rm1:SBopsem.rmetadata) 
-  (rm2:rmap) (lc1 lc2:GVMap) : Prop :=
-(forall i0 gv1, 
-  lookupAL _ lc1 i0 = Some gv1 -> 
-  exists gv2, 
-    lookupAL _ lc2 i0 = Some gv2 /\ gv_inject mi gv1 gv2
-) /\
-(forall vp bgv1 egv1, 
-  SBopsem.get_reg_metadata TD gl rm1 vp = 
-    Some (SBopsem.mkMD bgv1 egv1) -> 
-  exists bv2, exists ev2, exists bgv2, exists egv2,
-    get_reg_metadata rm2 vp = Some (bv2, ev2) /\
-    getOperandValue TD bv2 lc2 gl = Some bgv2 /\
-    getOperandValue TD ev2 lc2 gl = Some egv2 /\
-    gv_inject mi bgv1 bgv2 /\
-    gv_inject mi egv1 egv2
-).
-
-Fixpoint wf_global (maxb:Values.block) (gv:GenericValue) 
-  : Prop :=
-match gv with
-| nil => True
-| (Vptr b _,_)::gv' => b <= maxb /\ wf_global maxb gv'
-| _::gv' => wf_global maxb gv'
-end.
-
-Fixpoint wf_globals maxb (gl:GVMap) : Prop :=
-match gl with
-| nil => True
-| (_,gv)::gl' => wf_global maxb gv /\ wf_globals maxb gl'
-end.
-
-Definition mem_simulation (mi:Values.meminj) TD (max_gblock:Values.block) 
-  (MM1:SBopsem.mmetadata) (Mem1 Mem2:mem) : Prop :=
-Mem.mem_inj mi Mem1 Mem2 /\
-0 <= max_gblock < Mem.nextblock Mem2 /\
-(forall lc2 gl b ofs bgv egv als addrb addre bid0 eid0 pgv' fs F B cs tmn S Ps 
-    EC v,  
-  wf_globals max_gblock gl -> 
-  SBopsem.get_mem_metadata TD MM1 (ptr2GV TD (Vptr b ofs)) = 
-    SBopsem.mkMD bgv egv -> 
-  gv_inject mi (ptr2GV TD (Vptr b ofs)) pgv' ->
-  getOperandValue TD v lc2 gl = Some pgv' ->
-  exists bgv', exists egv',
-  LLVMopsem.dsop_star 
-    (LLVMopsem.mkState S TD Ps 
-      ((LLVMopsem.mkEC F B 
-        (insn_call bid0 false attrs gmb_typ gmb_fn
-           ((p8,v)::
-            (p8,(value_id addrb))::
-            (p8,(value_id addre))::nil)::
-         insn_call eid0 false attrs gmb_typ gmb_fn
-           ((p8,v)::
-            (p8,(value_id addrb))::
-            (p8,(value_id addre))::nil)::
-         cs) 
-        tmn lc2 als)
-        ::EC) gl fs Mem2)
-    (LLVMopsem.mkState S TD Ps 
-       ((LLVMopsem.mkEC F B cs tmn 
-         (updateAddAL _ (updateAddAL _ lc2 bid0 bgv') eid0 egv') als)::EC) 
-        gl fs Mem2)
-    trace_nil /\
-    gv_inject mi bgv bgv' /\
-    gv_inject mi egv egv'
-).
-
-Definition sbEC_simulates_EC_tail (TD:TargetData) gl (mi:Values.meminj) 
-  (sbEC:SBopsem.ExecutionContext) (EC:LLVMopsem.ExecutionContext) : Prop :=
-  match (sbEC, EC) with
-  | (SBopsem.mkEC f1 b1 ((insn_call i0 nr ca t0 v p)::cs13) tmn1 lc1 rm1 als1, 
-     LLVMopsem.mkEC f2 b2 cs2 tmn2 lc2 als2) =>
-       let '(fdef_intro fh1 bs1) := f1 in
-       let '(fdef_intro fh2 bs2) := f2 in
-       let '(los, nts) := TD in
-       trans_fdef nts f1 = Some f2 /\
-       tmn1 = tmn2 /\ als1 = als2 /\
-       (exists n, nth_error bs1 n = Some b1 /\ nth_error bs2 n = Some b2) /\
-       (exists l1, exists ps1, exists cs11, 
-         b1 = block_intro l1 ps1 (cs11++(insn_call i0 nr ca t0 v p)::cs13) tmn1)
-         /\
-       (exists l2, exists ps2, exists cs21,
-         b2 = block_intro l2 ps2 (cs21++cs2) tmn2) /\
-       exists ex_ids, exists rm2, 
-       exists ex_ids3, exists ex_ids4, exists cs22, exists cs23, exists cs24,
-         gen_metadata_fdef nts (getFdefLocs f1) nil f1 = Some (ex_ids, rm2) /\
-         reg_simulation mi TD gl rm1 rm2 lc1 lc2 /\
-         incl ex_ids ex_ids3 /\ 
-         call_suffix i0 nr ca t0 v p rm2 = Some cs22 /\
-         trans_cmds ex_ids3 rm2 cs13 = Some (ex_ids4,cs23) /\
-         trans_terminator rm2 tmn1 = Some cs24 /\
-         cs2 = cs22 ++ cs23 ++ cs24
-  | _ => False
-  end.
-
-Definition sbEC_simulates_EC_head (TD:TargetData) gl (mi:Values.meminj) 
-  (sbEC:SBopsem.ExecutionContext) (EC:LLVMopsem.ExecutionContext) : Prop :=
-  match (sbEC, EC) with
-  | (SBopsem.mkEC f1 b1 cs12 tmn1 lc1 rm1 als1, 
-     LLVMopsem.mkEC f2 b2 cs2 tmn2 lc2 als2) =>
-       let '(fdef_intro fh1 bs1) := f1 in
-       let '(fdef_intro fh2 bs2) := f2 in
-       let '(los, nts) := TD in
-       trans_fdef nts f1 = Some f2 /\
-       tmn1 = tmn2 /\ als1 = als2 /\
-       (exists n, nth_error bs1 n = Some b1 /\ nth_error bs2 n = Some b2) /\
-       (exists l1, exists ps1, exists cs11, 
-         b1 = block_intro l1 ps1 (cs11++cs12) tmn1) /\
-       (exists l2, exists ps2, exists cs21,
-         b2 = block_intro l2 ps2 (cs21++cs2) tmn2) /\
-       exists ex_ids, exists rm2, 
-       exists ex_ids3, exists ex_ids4, exists cs22, exists cs23,
-         gen_metadata_fdef nts (getFdefLocs f1) nil f1 = Some (ex_ids, rm2) /\
-         reg_simulation mi TD gl rm1 rm2 lc1 lc2 /\
-         incl ex_ids ex_ids3 /\ 
-         trans_cmds ex_ids3 rm2 cs12 = Some (ex_ids4,cs22) /\
-         trans_terminator rm2 tmn1 = Some cs23 /\
-         cs2 = cs22 ++ cs23
-  end.
-
-Fixpoint sbECs_simulate_ECs_tail (TD:TargetData) gl (mi:Values.meminj) 
-  (sbECs:SBopsem.ECStack) (ECs:LLVMopsem.ECStack) : Prop :=
-  match sbECs, ECs with
-  | nil, nil => True
-  | sbEC::sbECs', EC::ECs' => 
-      sbEC_simulates_EC_tail TD gl mi sbEC EC /\ 
-      sbECs_simulate_ECs_tail TD gl mi sbECs' ECs'
-  | _, _ => False
-  end.
-
-Definition sbECs_simulate_ECs (TD:TargetData) gl (mi:Values.meminj) 
-  (sbECs:SBopsem.ECStack) (ECs:LLVMopsem.ECStack) : Prop :=
-  match sbECs, ECs with
-  | sbEC::sbECs', EC::ECs' => 
-      sbEC_simulates_EC_head TD gl mi sbEC EC /\ 
-      sbECs_simulate_ECs_tail TD gl mi sbECs' ECs'
-  | _, _ => False
-  end.
-
-Definition sbState_simulates_State (mi:Values.meminj) (mgb:Values.block) 
-  (sbSt:SBopsem.State) (St:LLVMopsem.State) : Prop :=
-  match (sbSt, St) with
-  | (SBopsem.mkState S1 TD1 Ps1 ECs1 gl1 fs1 M1 MM1,
-     LLVMopsem.mkState S2 TD2 Ps2 ECs2 gl2 fs2 M2) =>
-      let '(los, nts) := TD1 in
-      trans_system S1 = Some S2 /\ 
-      TD1 = TD2 /\ 
-      trans_products nts Ps1 = trans_products nts Ps2 /\ 
-      sbECs_simulate_ECs TD1 gl1 mi ECs1 ECs2 /\
-      gl1 = gl2 /\ 
-      fs1 = fs2 /\ 
-      wf_sb_mi mgb mi M1 M2 /\
-      mem_simulation mi TD1 mgb MM1 M1 M2 
-  end.
-
-Lemma free_allocas_sim : forall TD M1 als M2 mi M1' MM mgb,
-  free_allocas TD M1 als = Some M1' ->
-  mem_simulation mi TD mgb MM M1 M2 ->
-  wf_sb_mi mgb mi M1 M2 ->
-  exists M2', free_allocas TD M2 als = Some M2' /\ 
-    mem_simulation mi TD mgb MM M1' M2' /\
-    wf_sb_mi mgb mi M1' M2'.
-Admitted.
-
-Definition sb_fnattrs := fnattrs_intro linkage_external visibility_default 
-  callconv_ccc nil nil.
-
-Axiom dstk_spec : forall M, 
-  LLVMopsem.callExternalFunction M dstk_fid nil = Some (None, M).
-
-Axiom dstk_is_found : forall TD Ps gl lc fs, 
-  LLVMopsem.lookupExFdecViaGV TD Ps gl lc fs dstk_fn = Some
-    (fdec_intro (fheader_intro sb_fnattrs dstk_typ dstk_fid nil false)).
-
-Definition int2GV n :=
-  (Vint 31 (Int.repr 31 (INTEGER.to_Z n)), AST.Mint 31)::nil.
-
-Axiom stk_ret_sim : forall TD M1 M2 mi MM mgb bgv egv,
-  mem_simulation mi TD mgb MM M1 M2 ->
-  wf_sb_mi mgb mi M1 M2 ->
-  exists M2',  exists M2'',
-    LLVMopsem.callExternalFunction M2 ssb_fid (bgv::int2GV 0%Z::nil) = 
-      Some (None, M2') /\
-    LLVMopsem.callExternalFunction M2' sse_fid (egv::int2GV 0%Z::nil) = 
-      Some (None, M2'') /\
-    mem_simulation mi TD mgb MM M1 M2'' /\
-    wf_sb_mi mgb mi M1 M2'' /\
-    LLVMopsem.callExternalFunction M2'' gsb_fid [int2GV 0%Z] = 
-      Some (Some bgv, M2'') /\
-    LLVMopsem.callExternalFunction M2'' gse_fid [int2GV 0%Z] = 
-      Some (Some egv, M2'').
-
-Axiom ssb_is_found : forall TD Ps gl lc fs, 
-  LLVMopsem.lookupExFdecViaGV TD Ps gl lc fs ssb_fn = Some
-    (fdec_intro (fheader_intro sb_fnattrs ssb_typ ssb_fid nil false)).
-
-Axiom sse_is_found : forall TD Ps gl lc fs, 
-  LLVMopsem.lookupExFdecViaGV TD Ps gl lc fs sse_fn = Some
-    (fdec_intro (fheader_intro sb_fnattrs sse_typ sse_fid nil false)).
-
-Axiom gsb_is_found : forall TD Ps gl lc fs, 
-  LLVMopsem.lookupExFdecViaGV TD Ps gl lc fs gsb_fn = Some
-    (fdec_intro (fheader_intro sb_fnattrs gsb_typ gsb_fid nil false)).
-
-Axiom gse_is_found : forall TD Ps gl lc fs, 
-  LLVMopsem.lookupExFdecViaGV TD Ps gl lc fs gse_fn = Some
-    (fdec_intro (fheader_intro sb_fnattrs gse_typ gse_fid nil false)).
-
-Lemma SBpass_is_correct : forall mi mgb sbSt St sbSt' tr,
-  sbState_simulates_State mi mgb sbSt St ->
-  SBopsem.dsInsn sbSt sbSt' tr -> 
-  exists St', exists mi',
-    LLVMopsem.dsop_star St St' tr /\    
-    sbState_simulates_State mi' mgb sbSt' St' /\
-    Values.inject_incr mi mi'.
-Proof.
-  intros mi mgb sbSt St sbSt' tr Hsim Hsbop.
-  (sb_dsInsn_cases (induction Hsbop) Case).
-Case "dsReturn". Focus.
-  destruct St as [S2 TD2 Ps2 ECs2 gl2 fs2 M2].
-  destruct TD as [los nts].
-  destruct Hsim as [Htsym [Heq1 [Htps [HsimECs [Heq2 [Heq3 [Hwfmi HsimM]]]]]]];
-    subst.
+Ltac destruct_ctx_return :=
+match goal with
+| [Hsim : sbState_simulates_State _ _
+           {|
+           SBopsem.CurSystem := _;
+           SBopsem.CurTargetData := ?TD;
+           SBopsem.CurProducts := _;
+           SBopsem.ECS := {|
+                          SBopsem.CurFunction := ?F;
+                          SBopsem.CurBB := _;
+                          SBopsem.CurCmds := nil;
+                          SBopsem.Terminator := _;
+                          SBopsem.Locals := _;
+                          SBopsem.Rmap := _;
+                          SBopsem.Allocas := _ |}
+                          :: {|
+                             SBopsem.CurFunction := ?F';
+                             SBopsem.CurBB := _;
+                             SBopsem.CurCmds := ?c' :: _;
+                             SBopsem.Terminator := _;
+                             SBopsem.Locals := _;
+                             SBopsem.Rmap := _;
+                             SBopsem.Allocas := _ |} :: _;
+           SBopsem.Globals := _;
+           SBopsem.FunTable := _;
+           SBopsem.Mem := _;
+           SBopsem.Mmap := _ |} ?St |- _] =>
+  destruct St as [S2 TD2 Ps2 ECs2 gl2 fs2 M2];
+  destruct TD as [los nts];
+  destruct Hsim as [Hwfs [HMinS [Htsym [Heq1 [Htps [HsimECs [Heq2 [Heq3 [Hwfg 
+    [Hwfmi HsimM]]]]]]]]]];
+    subst;
   destruct ECs2 as [|[F2 B2 cs2 tmn2 lc2 als2] ECs2];
-    try solve [inversion HsimECs].
-  simpl in HsimECs.
-  destruct HsimECs as [HsimEC HsimECs].
+    try solve [inversion HsimECs];
+  simpl in HsimECs;
+  destruct HsimECs as [HsimEC HsimECs];
   destruct ECs2 as [|[F2' B2' cs2' tmn2' lc2' als2'] ECs2];
-    try solve [inversion HsimECs].
-  destruct HsimECs as [HsimEC' HsimECs].
-  destruct F as [fh1 bs1].
-  destruct F2 as [fh2 bs2].
-  destruct HsimEC as [Htfdef [Heq0 [Heq1 [Hnth [Heqb1 [Heqb2 [ex_ids [rm2 
-    [ex_ids3 [ex_ids4 [cs22 [cs23 [Hgenmeta [Hrsim 
-    [Hinc [Htcmds [Httmn Heq2]]]]]]]]]]]]]]]]]; subst.
-  destruct F' as [fh1' bs1'].
-  destruct F2' as [fh2' bs2'].
-  destruct c'; try solve [inversion HsimEC'].  
-  destruct HsimEC' as [Htfdef' [Heq0' [Heq1' [Hnth' [Heqb1' [Heqb2'
-    [ex_ids' [rm2' [ex_ids3' [ex_ids4' [cs22' [cs23' [cs24' 
-    [Hgenmeta' [Hrsim' [Hinc' [Hcall' [Htcmds' [Httmn' Heq2']]]]]]]]]]]]]]]]]]]; 
-    subst.
+    try solve [inversion HsimECs];
+  destruct HsimECs as [HsimEC' HsimECs];
+  destruct F as [fh1 bs1];
+  destruct F2 as [fh2 bs2];
+  destruct HsimEC as [HBinF [HFinPs [Htfdef [Heq0 [Hasim [Hnth [Heqb1 [Heqb2 
+    [ex_ids [rm2 [ex_ids3 [ex_ids4 [cs22 [cs23 [Hgenmeta [Hrsim [Hinc [Hfresh 
+    [Htcmds [Httmn Heq2]]]]]]]]]]]]]]]]]]]]; subst;
+  destruct F' as [fh1' bs1'];
+  destruct F2' as [fh2' bs2'];
+  destruct c'; try solve [inversion HsimEC'];
+  destruct HsimEC' as [HBinF' [HFinPs' [Htfdef' [Heq0' [Hasim' [Hnth' [Heqb1' 
+    [Heqb2' [ex_ids' [rm2' [ex_ids3' [ex_ids4' [cs22' [cs23' [cs24' 
+    [Hgenmeta' [Hrsim' [Hinc' [Hcall' [Hfresh' [Htcmds' [Httmn' Heq2']]]]]]]]]]]]
+    ]]]]]]]]]]; 
+    subst
+end.
+
+Lemma SBpass_is_correct__dsReturn : forall 
+  (mi : meminj)
+  (mgb : Values.block)
+  (St : LLVMopsem.State)
+  (S : system)
+  (TD : TargetData)
+  (Ps : list product)
+  (F : fdef)
+  (B : block)
+  (rid : id)
+  (RetTy : typ)
+  (Result : value)
+  (lc : GVMap)
+  (rm : SBopsem.rmetadata)
+  (gl : GVMap)
+  (fs : GVMap)
+  (F' : fdef)
+  (B' : block)
+  (c' : cmd)
+  (cs' : list cmd)
+  (tmn' : terminator)
+  (lc' : GVMap)
+  (rm' : SBopsem.rmetadata)
+  (EC : list SBopsem.ExecutionContext)
+  (Mem : mem)
+  (MM : SBopsem.mmetadata)
+  (als : list mblock)
+  (als' : list mblock)
+  (Hsim : sbState_simulates_State mi mgb
+           {|
+           SBopsem.CurSystem := S;
+           SBopsem.CurTargetData := TD;
+           SBopsem.CurProducts := Ps;
+           SBopsem.ECS := {|
+                          SBopsem.CurFunction := F;
+                          SBopsem.CurBB := B;
+                          SBopsem.CurCmds := nil;
+                          SBopsem.Terminator := insn_return rid RetTy Result;
+                          SBopsem.Locals := lc;
+                          SBopsem.Rmap := rm;
+                          SBopsem.Allocas := als |}
+                          :: {|
+                             SBopsem.CurFunction := F';
+                             SBopsem.CurBB := B';
+                             SBopsem.CurCmds := c' :: cs';
+                             SBopsem.Terminator := tmn';
+                             SBopsem.Locals := lc';
+                             SBopsem.Rmap := rm';
+                             SBopsem.Allocas := als' |} :: EC;
+           SBopsem.Globals := gl;
+           SBopsem.FunTable := fs;
+           SBopsem.Mem := Mem;
+           SBopsem.Mmap := MM |} St)
+  (Mem' : mem)
+  (lc'' : GVMap)
+  (rm'' : SBopsem.rmetadata)
+  (H : Instruction.isCallInst c' = true)
+  (H0 : free_allocas TD Mem als = ret Mem')
+  (H1 : SBopsem.returnUpdateLocals TD c' RetTy Result lc lc' rm rm' gl =
+       ret (lc'', rm'')),
+  exists St' : LLVMopsem.State,
+     exists mi' : meminj,
+       LLVMopsem.dsop_star St St' trace_nil /\
+       sbState_simulates_State mi' mgb
+         {|
+         SBopsem.CurSystem := S;
+         SBopsem.CurTargetData := TD;
+         SBopsem.CurProducts := Ps;
+         SBopsem.ECS := {|
+                        SBopsem.CurFunction := F';
+                        SBopsem.CurBB := B';
+                        SBopsem.CurCmds := cs';
+                        SBopsem.Terminator := tmn';
+                        SBopsem.Locals := lc'';
+                        SBopsem.Rmap := rm'';
+                        SBopsem.Allocas := als' |} :: EC;
+         SBopsem.Globals := gl;
+         SBopsem.FunTable := fs;
+         SBopsem.Mem := Mem';
+         SBopsem.Mmap := MM |} St' /\ inject_incr mi mi'.
+Proof.
+  intros.
+  destruct_ctx_return.
   inv Htcmds.
   simpl in H1.
   unfold call_suffix in Hcall'.
@@ -318,7 +176,7 @@ Case "dsReturn". Focus.
     inv H1.
     simpl in Httmn.
     destruct (isPointerTypB RetTy).
-    SSCase "rt is ptr". Focus.
+    SSCase "rt is ptr". 
       remember (SBopsem.get_reg_metadata (los, nts) gl2 rm Result) as oRmd.
       destruct oRmd as [[bgv1 egv1]|]; inv HeqRet.
       assert (exists bv2, exists ev2, exists bgv2, exists egv2,
@@ -332,15 +190,11 @@ Case "dsReturn". Focus.
         apply Hrsim; auto.
       destruct J as [bv2 [ev2 [bgv2 [egv2 [Hgetrmd [Hgetbgv2 [Hgetegv2 [Hinj1 
         Hinj2]]]]]]]]. rewrite Hgetrmd in Httmn. inv Httmn.
-Admitted.
-(*
-      destruct (@stk_ret_sim (los,nts) Mem M2 mi MM mgb lc'' lc2' rm'' rm2'
-        gl2 EC ECs2 bv null) as [M2' [M2'' [Hsbase [Hsbound [Hmsim3 [Hrsim3
-        [HsimECs3 [Hwfmi3 [Hgbase Hgbound]]]]]]]]]; auto.
-      eapply free_allocas_sim with (rm1:=rm'')(rm2:=rm2')(lc1:=lc'')(lc2:=lc2') 
-        in HsimECs3; eauto.
-      destruct HsimECs3 as [M2''' [Hfree2' [Hmsim2' [Hrsim2' [HsimECs2' Hwfmi2']]
-        ]]].
+      destruct (@stk_ret_sim (los,nts) Mem0 M2 mi mgb MM bgv2 egv2) as 
+        [M2' [M2'' [Hsbase [Hsbound [Hmsim3 [Hwfmi3 [Hgbase Hgbound]]]]]]]; 
+        auto.
+      eapply free_allocas_sim in Hmsim3; eauto.
+      destruct Hmsim3 as [M2''' [Hfree2' [Hmsim2' Hwfmi2']]].
       exists (LLVMopsem.mkState S2 (los, nts) Ps2
         ((LLVMopsem.mkEC (fdef_intro fh2' bs2') B2'
             (cs23' ++ cs24') tmn2' lc2' als2'):: ECs2)
@@ -352,8 +206,8 @@ Admitted.
         apply LLVMopsem.dsop_star_cons with (state2:=
           (LLVMopsem.mkState S2 (los, nts) Ps2
             ((LLVMopsem.mkEC (fdef_intro fh2 bs2) B2
-              ((insn_call fake_id true attrs sbound_typ sbound_fn 
-                  ((p8, vnullp8)::(i32, vint0) :: nil))::nil)
+              ((insn_call fake_id true attrs sse_typ sse_fn 
+                  ((p8, ev2)::(i32, vint0) :: nil))::nil)
               (insn_return rid RetTy Result) lc2 als2)::
              (LLVMopsem.mkEC (fdef_intro fh2' bs2') B2'
               ((insn_call i0 true c t (wrap_call v) p)::
@@ -361,9 +215,11 @@ Admitted.
               (cs23' ++ cs24'))
               tmn2' lc2' als2'):: ECs2)
             gl2 fs2 M2')).
-          eapply LLVMopsem.dsExCall with (fid:=sbase_fid)
-            (gvs:=(null :: int2GV 0 :: nil))(oresult:=None); eauto.
-            eapply sbase_is_found; eauto.
+          eapply LLVMopsem.dsExCall with (fid:=ssb_fid)
+            (gvs:=(bgv2 :: int2GV 0 :: nil))(oresult:=None); eauto.
+            eapply ssb_is_found; eauto.
+            simpl. rewrite Hgetbgv2. auto.
+
         rewrite <- (@trace_app_nil__eq__trace trace_nil).
         apply LLVMopsem.dsop_star_cons with (state2:=
           (LLVMopsem.mkState S2 (los, nts) Ps2
@@ -375,9 +231,11 @@ Admitted.
               (cs23' ++ cs24'))
               tmn2' lc2' als2'):: ECs2)
             gl2 fs2 M2'')).
-          eapply LLVMopsem.dsExCall with (fid:=sbound_fid)
-            (gvs:=(null :: int2GV 0 :: nil))(oresult:=None); eauto.
-            eapply sbound_is_found; eauto.
+          eapply LLVMopsem.dsExCall with (fid:=sse_fid)
+            (gvs:=(egv2 :: int2GV 0 :: nil))(oresult:=None); eauto.
+            eapply sse_is_found; eauto.
+            simpl. rewrite Hgetegv2. auto.
+
         rewrite <- (@trace_app_nil__eq__trace trace_nil).
         apply LLVMopsem.dsop_star_cons with (state2:=
           (LLVMopsem.mkState S2 (los, nts) Ps2
@@ -387,6 +245,12 @@ Admitted.
               tmn2' lc2' als2'):: ECs2)
             gl2 fs2 M2''')).
           eapply LLVMopsem.dsReturn; eauto.
+            unfold LLVMopsem.returnUpdateLocals. simpl.
+            clear - Hrsim Heqogr Hwfg Hwfmi.
+            symmetry in Heqogr.
+            eapply simulation__getOperandValue in Heqogr; eauto.
+            destruct Heqogr as [gv' [J1 J2]]. rewrite J1. auto.
+
         rewrite <- (@trace_app_nil__eq__trace trace_nil).
         apply LLVMopsem.dsop_star_cons with (state2:=
           (LLVMopsem.mkState S2 (los, nts) Ps2
@@ -401,10 +265,7 @@ Admitted.
       split; auto using inject_incr_refl.
       SSSCase "sim".
       repeat (split; auto).
-          destruct Heqb1' as [l1' [ps1' [cs11' Heqb1']]]; subst.
-          exists l1'. exists ps1'. 
-          exists (cs11' ++ [insn_call i0 true c t v p]). 
-          simpl_env. auto.
+          eapply cmds_at_block_tail_next; eauto.
 
           destruct Heqb2' as [l2' [ps2' [cs21' Heqb2']]]; subst.
           exists l2'. exists ps2'. exists (cs21' ++
@@ -413,20 +274,16 @@ Admitted.
           simpl_env. auto.
  
           exists ex_ids'. exists rm2'.
-          exists addrb'. exists ex_ids1'. exists addre'. exists ex_ids2'. 
           exists ex_ids3'. exists ex_ids4'. exists cs23'. exists cs24'.
           repeat (split; auto).
 
-
     SSCase "rt isnt ptr".
       inv Httmn.
-      destruct (@stk_ret_sim (los,nts) Mem M2 mi MM mgb lc'' lc2' rm'' rm2'
-        gl2 EC ECs2 null null) as [M2' [M2'' [Hsbase [Hsbound [Hmsim3 [Hrsim3
-        [HsimECs3 [Hwfmi3 [Hgbase Hgbound]]]]]]]]]; auto.
-      eapply free_allocas_sim with (rm1:=rm'')(rm2:=rm2')(lc1:=lc'')(lc2:=lc2') 
-        in HsimECs3; eauto.
-      destruct HsimECs3 as [M2''' [Hfree2' [Hmsim2' [Hrsim2' [HsimECs2' Hwfmi2']]
-        ]]].
+      destruct (@stk_ret_sim (los,nts) Mem0 M2 mi mgb MM null null) as 
+        [M2' [M2'' [Hsbase [Hsbound [Hmsim3 [Hwfmi3 [Hgbase Hgbound]]]]]]]; 
+        auto.
+      eapply free_allocas_sim in Hmsim3; eauto.
+      destruct Hmsim3 as [M2''' [Hfree2' [Hmsim2' Hwfmi2']]].
       exists (LLVMopsem.mkState S2 (los, nts) Ps2
         ((LLVMopsem.mkEC (fdef_intro fh2' bs2') B2'
             (cs23' ++ cs24') tmn2' lc2' als2'):: ECs2)
@@ -438,7 +295,7 @@ Admitted.
         apply LLVMopsem.dsop_star_cons with (state2:=
           (LLVMopsem.mkState S2 (los, nts) Ps2
             ((LLVMopsem.mkEC (fdef_intro fh2 bs2) B2
-              ((insn_call fake_id true attrs sbound_typ sbound_fn 
+              ((insn_call fake_id true attrs sse_typ sse_fn 
                   ((p8, vnullp8)::(i32, vint0) :: nil))::nil)
               (insn_return rid RetTy Result) lc2 als2)::
              (LLVMopsem.mkEC (fdef_intro fh2' bs2') B2'
@@ -447,9 +304,9 @@ Admitted.
               (cs23' ++ cs24'))
               tmn2' lc2' als2'):: ECs2)
             gl2 fs2 M2')).
-          eapply LLVMopsem.dsExCall with (fid:=sbase_fid)
+          eapply LLVMopsem.dsExCall with (fid:=ssb_fid)
             (gvs:=(null :: int2GV 0 :: nil))(oresult:=None); eauto.
-            eapply sbase_is_found; eauto.
+            eapply ssb_is_found; eauto.
         rewrite <- (@trace_app_nil__eq__trace trace_nil).
         apply LLVMopsem.dsop_star_cons with (state2:=
           (LLVMopsem.mkState S2 (los, nts) Ps2
@@ -461,9 +318,9 @@ Admitted.
               (cs23' ++ cs24'))
               tmn2' lc2' als2'):: ECs2)
             gl2 fs2 M2'')).
-          eapply LLVMopsem.dsExCall with (fid:=sbound_fid)
+          eapply LLVMopsem.dsExCall with (fid:=sse_fid)
             (gvs:=(null :: int2GV 0 :: nil))(oresult:=None); eauto.
-            eapply sbound_is_found; eauto.
+            eapply sse_is_found; eauto.
         rewrite <- (@trace_app_nil__eq__trace trace_nil).
         apply LLVMopsem.dsop_star_cons with (state2:=
           (LLVMopsem.mkState S2 (los, nts) Ps2
@@ -473,6 +330,12 @@ Admitted.
               tmn2' lc2' als2'):: ECs2)
             gl2 fs2 M2''')).
           eapply LLVMopsem.dsReturn; eauto.
+            unfold LLVMopsem.returnUpdateLocals. simpl.
+            clear - Hrsim Heqogr Hwfg Hwfmi.
+            symmetry in Heqogr.
+            eapply simulation__getOperandValue in Heqogr; eauto.
+            destruct Heqogr as [gv' [J1 J2]]. rewrite J1. auto.
+
         rewrite <- (@trace_app_nil__eq__trace trace_nil).
         apply LLVMopsem.dsop_star_cons with (state2:=
           (LLVMopsem.mkState S2 (los, nts) Ps2
@@ -487,10 +350,7 @@ Admitted.
       split; auto using inject_incr_refl.
       SSSCase "sim".
       repeat (split; auto).
-          destruct Heqb1' as [l1' [ps1' [cs11' Heqb1']]]; subst.
-          exists l1'. exists ps1'. 
-          exists (cs11' ++ [insn_call i0 true c t v p]). 
-          simpl_env. auto.
+          eapply cmds_at_block_tail_next; eauto.
 
           destruct Heqb2' as [l2' [ps2' [cs21' Heqb2']]]; subst.
           exists l2'. exists ps2'. exists (cs21' ++
@@ -499,110 +359,2381 @@ Admitted.
           simpl_env. auto.
  
           exists ex_ids'. exists rm2'.
-          exists addrb'. exists ex_ids1'. exists addre'. exists ex_ids2'. 
           exists ex_ids3'. exists ex_ids4'. exists cs23'. exists cs24'.
           repeat (split; auto).
 
   SCase "nret = false".
-    remember (getOperandValue (los, nts) Mem' Result lc gl2) as R.
-    destruct R; try solve [inv H1].
-    destruct (SBopsem.isReturnPointerTypB t); simpl in Hcall'.
+    destruct (SBopsem.isReturnPointerTypB t).
     SSCase "ct is ptr".
+      simpl in Hcall'.
+      remember (lookupAL (id * id) rm2' i0) as R.
+      destruct R as [[bid0 eid0]|]; inv Hcall'.
       simpl in Httmn.
       destruct (isPointerTypB RetTy).
-    SSSCase "rt is ptr".
-      destruct (get_reg_metadata rm2 Result) as [[bv ev]|]; inv Httmn.
-
-
-
-    inv H1.
-    inv Hcall'.
-
-    SSCase "rt isnt ptr".
-      inv Httmn.
-      destruct (@stk_ret_sim (los,nts) Mem M2 mi MM mgb lc'' lc2' rm'' rm2'
-        gl2 EC ECs2 null null) as [M2' [M2'' [Hsbase [Hsbound [Hmsim3 [Hrsim3
-        [HsimECs3 [Hwfmi3 [Hgbase Hgbound]]]]]]]]]; auto.
-      eapply free_allocas_sim with (rm1:=rm'')(rm2:=rm2')(lc1:=lc'')(lc2:=lc2') 
-        in HsimECs3; eauto.
-      destruct HsimECs3 as [M2''' [Hfree2' [Hmsim2' [Hrsim2' [HsimECs2' Hwfmi2']]
-        ]]].
+    SSSCase "rt is ptr". 
+      inv H1.
+      remember (SBopsem.get_reg_metadata (los, nts) gl2 rm Result) as oRmd.
+      destruct oRmd as [[bgv1 egv1]|]; inv HeqRet.
+      assert (exists bv2, exists ev2, exists bgv2, exists egv2,
+        get_reg_metadata rm2 Result = Some (bv2, ev2) /\
+        getOperandValue (los,nts) bv2 lc2 gl2 = Some bgv2 /\
+        getOperandValue (los,nts) ev2 lc2 gl2 = Some egv2 /\
+        gv_inject mi bgv1 bgv2 /\
+        gv_inject mi egv1 egv2) as J.
+        clear - HeqoRmd Hrsim. 
+        destruct Hrsim as [_ Hrsim].
+        apply Hrsim; auto.
+      destruct J as [bv2 [ev2 [bgv2 [egv2 [Hgetrmd [Hgetbgv2 [Hgetegv2 [Hinj1 
+        Hinj2]]]]]]]]. rewrite Hgetrmd in Httmn. inv Httmn.
+      destruct (@stk_ret_sim (los,nts) Mem0 M2 mi mgb MM bgv2 egv2) as 
+        [M2' [M2'' [Hsbase [Hsbound [Hmsim3 [Hwfmi3 [Hgbase Hgbound]]]]]]]; 
+        auto.
+      eapply free_allocas_sim in Hmsim3; eauto.
+      destruct Hmsim3 as [M2''' [Hfree2' [Hmsim2' Hwfmi2']]].
+      symmetry in Heqogr.
+      eapply simulation__getOperandValue in Heqogr; eauto.
+      destruct Heqogr as [gr2 [J1 J2]]. 
       exists (LLVMopsem.mkState S2 (los, nts) Ps2
         ((LLVMopsem.mkEC (fdef_intro fh2' bs2') B2'
-            (cs23' ++ cs24') tmn2' lc2' als2'):: ECs2)
+            (cs23' ++ cs24') tmn2' 
+            (updateAddAL _ (updateAddAL _ (updateAddAL _ lc2' i0 gr2) bid0 bgv2) 
+              eid0 egv2)
+            als2'):: ECs2)
         gl2 fs2 M2''').
       exists mi.
       split.
-      SSSCase "dsop_star".
+      SSSSCase "dsop_star".
         rewrite <- (@trace_app_nil__eq__trace trace_nil).
         apply LLVMopsem.dsop_star_cons with (state2:=
           (LLVMopsem.mkState S2 (los, nts) Ps2
             ((LLVMopsem.mkEC (fdef_intro fh2 bs2) B2
-              ((insn_call fake_id true attrs sbound_typ sbound_fn 
-                  ((p8, vnullp8)::(i32, vint0) :: nil))::nil)
+              ((insn_call fake_id true attrs sse_typ sse_fn 
+                  ((p8, ev2)::(i32, vint0) :: nil))::nil)
               (insn_return rid RetTy Result) lc2 als2)::
              (LLVMopsem.mkEC (fdef_intro fh2' bs2') B2'
-              ((insn_call i0 true c t (wrap_call v) p)::
+              ((insn_call i0 false c t (wrap_call v) p)::
+               insn_call bid0 false attrs gsb_typ gsb_fn((i32, vint0) :: nil):: 
+               insn_call eid0 false attrs gse_typ gse_fn((i32, vint0) :: nil)::
                (insn_call fake_id true attrs dstk_typ dstk_fn nil)::
-              (cs23' ++ cs24'))
+               cs23' ++ cs24')
               tmn2' lc2' als2'):: ECs2)
-            gl2 fs2 M2')).
-          eapply LLVMopsem.dsExCall with (fid:=sbase_fid)
-            (gvs:=(null :: int2GV 0 :: nil))(oresult:=None); eauto.
-            eapply sbase_is_found; eauto.
+            gl2 fs2 M2')). 
+          eapply LLVMopsem.dsExCall with (fid:=ssb_fid)
+            (gvs:=(bgv2 :: int2GV 0 :: nil))(oresult:=None); eauto.
+            eapply ssb_is_found; eauto.
+            simpl. rewrite Hgetbgv2. auto.
+
         rewrite <- (@trace_app_nil__eq__trace trace_nil).
         apply LLVMopsem.dsop_star_cons with (state2:=
           (LLVMopsem.mkState S2 (los, nts) Ps2
             ((LLVMopsem.mkEC (fdef_intro fh2 bs2) B2 nil
               (insn_return rid RetTy Result) lc2 als2)::
              (LLVMopsem.mkEC (fdef_intro fh2' bs2') B2'
-              ((insn_call i0 true c t (wrap_call v) p)::
+              ((insn_call i0 false c t (wrap_call v) p)::
+               insn_call bid0 false attrs gsb_typ gsb_fn((i32, vint0) :: nil):: 
+               insn_call eid0 false attrs gse_typ gse_fn((i32, vint0) :: nil)::
                (insn_call fake_id true attrs dstk_typ dstk_fn nil)::
               (cs23' ++ cs24'))
               tmn2' lc2' als2'):: ECs2)
             gl2 fs2 M2'')).
-          eapply LLVMopsem.dsExCall with (fid:=sbound_fid)
-            (gvs:=(null :: int2GV 0 :: nil))(oresult:=None); eauto.
-            eapply sbound_is_found; eauto.
+          eapply LLVMopsem.dsExCall with (fid:=sse_fid)
+            (gvs:=(egv2 :: int2GV 0 :: nil))(oresult:=None); eauto.
+            eapply sse_is_found; eauto.
+            simpl. rewrite Hgetegv2. auto.
+
         rewrite <- (@trace_app_nil__eq__trace trace_nil).
         apply LLVMopsem.dsop_star_cons with (state2:=
           (LLVMopsem.mkState S2 (los, nts) Ps2
             ((LLVMopsem.mkEC (fdef_intro fh2' bs2') B2'
-              ((insn_call fake_id true attrs dstk_typ dstk_fn nil)::
-              (cs23' ++ cs24'))
-              tmn2' lc2' als2'):: ECs2)
+              (insn_call bid0 false attrs gsb_typ gsb_fn((i32, vint0) :: nil):: 
+               insn_call eid0 false attrs gse_typ gse_fn((i32, vint0) :: nil)::
+               insn_call fake_id true attrs dstk_typ dstk_fn nil::
+               (cs23' ++ cs24'))
+              tmn2' (updateAddAL _ lc2' i0 gr2) als2'):: ECs2)
             gl2 fs2 M2''')).
           eapply LLVMopsem.dsReturn; eauto.
+            unfold LLVMopsem.returnUpdateLocals. simpl.
+            rewrite J1. auto.
+
+        rewrite <- (@trace_app_nil__eq__trace trace_nil).
+        apply LLVMopsem.dsop_star_cons with (state2:=
+          (LLVMopsem.mkState S2 (los, nts) Ps2
+            ((LLVMopsem.mkEC (fdef_intro fh2' bs2') B2'
+              (insn_call eid0 false attrs gse_typ gse_fn((i32, vint0) :: nil)::
+               insn_call fake_id true attrs dstk_typ dstk_fn nil::
+               (cs23' ++ cs24'))
+              tmn2' (updateAddAL _ (updateAddAL _ lc2' i0 gr2) bid0 bgv2) 
+              als2'):: ECs2)
+            gl2 fs2 M2''')).
+          eapply LLVMopsem.dsExCall with (fid:=gsb_fid)
+            (gvs:=(int2GV 0 :: nil))(oresult:=Some bgv2); eauto.
+            eapply gsb_is_found; eauto.
+              clear - Hfree2' Hgbase.
+              eapply free_doesnt_change_gsb; eauto.
+
+        rewrite <- (@trace_app_nil__eq__trace trace_nil).
+        apply LLVMopsem.dsop_star_cons with (state2:=
+          (LLVMopsem.mkState S2 (los, nts) Ps2
+            ((LLVMopsem.mkEC (fdef_intro fh2' bs2') B2'
+              (insn_call fake_id true attrs dstk_typ dstk_fn nil:: 
+               cs23' ++ cs24')
+              tmn2' (updateAddAL _ (updateAddAL _ (updateAddAL _ lc2' i0 gr2) 
+                bid0 bgv2) eid0 egv2) als2'):: ECs2)
+            gl2 fs2 M2''')); auto.
+          eapply LLVMopsem.dsExCall with (fid:=gse_fid)
+            (gvs:=(int2GV 0 :: nil))(oresult:=Some egv2); eauto.
+            eapply gse_is_found; eauto.
+              clear - Hfree2' Hgbound.
+              eapply free_doesnt_change_gse; eauto.
+
         rewrite <- (@trace_app_nil__eq__trace trace_nil).
         apply LLVMopsem.dsop_star_cons with (state2:=
           (LLVMopsem.mkState S2 (los, nts) Ps2
             ((LLVMopsem.mkEC (fdef_intro fh2' bs2') B2'
               (cs23' ++ cs24')
-              tmn2' lc2' als2'):: ECs2)
+              tmn2' (updateAddAL _ (updateAddAL _ (updateAddAL _ lc2' i0 gr2) 
+                bid0 bgv2) eid0 egv2) als2'):: ECs2)
             gl2 fs2 M2''')); auto.
           eapply LLVMopsem.dsExCall; simpl; eauto.
             eapply dstk_is_found; eauto.
             eapply dstk_spec; eauto.
 
       split; auto using inject_incr_refl.
-      SSSCase "sim".
+      SSSSCase "sim".
       repeat (split; auto).
-          destruct Heqb1' as [l1' [ps1' [cs11' Heqb1']]]; subst.
-          exists l1'. exists ps1'. 
-          exists (cs11' ++ [insn_call i0 true c t v p]). 
-          simpl_env. auto.
+          eapply cmds_at_block_tail_next; eauto.
 
           destruct Heqb2' as [l2' [ps2' [cs21' Heqb2']]]; subst.
           exists l2'. exists ps2'. exists (cs21' ++
-              [insn_call i0 true c t (wrap_call v) p] ++
+              [insn_call i0 false c t (wrap_call v) p] ++
+              [insn_call bid0 false attrs gsb_typ gsb_fn [(i32, vint0)]] ++
+              [insn_call eid0 false attrs gse_typ gse_fn [(i32, vint0)]] ++
               [insn_call fake_id true attrs dstk_typ dstk_fn nil]). 
           simpl_env. auto.
  
           exists ex_ids'. exists rm2'.
-          exists addrb'. exists ex_ids1'. exists addre'. exists ex_ids2'. 
           exists ex_ids3'. exists ex_ids4'. exists cs23'. exists cs24'.
-          repeat (split; auto).
-*)
+          repeat (split; auto).              
+            clear - J2 Hrsim' HeqR. admit.
+            clear - J2 Hrsim' HeqR Hinj1 Hinj2. admit.
+
+    SSSCase "rt isnt ptr". 
+      inv H1. inv HeqRet. inv Httmn.
+      destruct (@stk_ret_sim (los,nts) Mem0 M2 mi mgb MM null null) as 
+        [M2' [M2'' [Hsbase [Hsbound [Hmsim3 [Hwfmi3 [Hgbase Hgbound]]]]]]]; 
+        auto.
+      eapply free_allocas_sim in Hmsim3; eauto.
+      destruct Hmsim3 as [M2''' [Hfree2' [Hmsim2' Hwfmi2']]].
+      symmetry in Heqogr.
+      eapply simulation__getOperandValue in Heqogr; eauto.
+      destruct Heqogr as [gr2 [J1 J2]]. 
+      exists (LLVMopsem.mkState S2 (los, nts) Ps2
+        ((LLVMopsem.mkEC (fdef_intro fh2' bs2') B2'
+            (cs23' ++ cs24') tmn2' 
+            (updateAddAL _ (updateAddAL _ (updateAddAL _ lc2' i0 gr2) bid0 null) 
+              eid0 null)
+            als2'):: ECs2)
+        gl2 fs2 M2''').
+      exists mi.
+      split.
+      SSSSCase "dsop_star".
+        rewrite <- (@trace_app_nil__eq__trace trace_nil).
+        apply LLVMopsem.dsop_star_cons with (state2:=
+          (LLVMopsem.mkState S2 (los, nts) Ps2
+            ((LLVMopsem.mkEC (fdef_intro fh2 bs2) B2
+              ((insn_call fake_id true attrs sse_typ sse_fn 
+                  ((p8, vnullp8)::(i32, vint0) :: nil))::nil)
+              (insn_return rid RetTy Result) lc2 als2)::
+             (LLVMopsem.mkEC (fdef_intro fh2' bs2') B2'
+              ((insn_call i0 false c t (wrap_call v) p)::
+               insn_call bid0 false attrs gsb_typ gsb_fn((i32, vint0) :: nil):: 
+               insn_call eid0 false attrs gse_typ gse_fn((i32, vint0) :: nil)::
+               (insn_call fake_id true attrs dstk_typ dstk_fn nil)::
+               cs23' ++ cs24')
+              tmn2' lc2' als2'):: ECs2)
+            gl2 fs2 M2')). 
+          eapply LLVMopsem.dsExCall with (fid:=ssb_fid)
+            (gvs:=(null :: int2GV 0 :: nil))(oresult:=None); eauto.
+            eapply ssb_is_found; eauto.
+
+        rewrite <- (@trace_app_nil__eq__trace trace_nil).
+        apply LLVMopsem.dsop_star_cons with (state2:=
+          (LLVMopsem.mkState S2 (los, nts) Ps2
+            ((LLVMopsem.mkEC (fdef_intro fh2 bs2) B2 nil
+              (insn_return rid RetTy Result) lc2 als2)::
+             (LLVMopsem.mkEC (fdef_intro fh2' bs2') B2'
+              ((insn_call i0 false c t (wrap_call v) p)::
+               insn_call bid0 false attrs gsb_typ gsb_fn((i32, vint0) :: nil):: 
+               insn_call eid0 false attrs gse_typ gse_fn((i32, vint0) :: nil)::
+               (insn_call fake_id true attrs dstk_typ dstk_fn nil)::
+              (cs23' ++ cs24'))
+              tmn2' lc2' als2'):: ECs2)
+            gl2 fs2 M2'')).
+          eapply LLVMopsem.dsExCall with (fid:=sse_fid)
+            (gvs:=(null :: int2GV 0 :: nil))(oresult:=None); eauto.
+            eapply sse_is_found; eauto.
+
+        rewrite <- (@trace_app_nil__eq__trace trace_nil).
+        apply LLVMopsem.dsop_star_cons with (state2:=
+          (LLVMopsem.mkState S2 (los, nts) Ps2
+            ((LLVMopsem.mkEC (fdef_intro fh2' bs2') B2'
+              (insn_call bid0 false attrs gsb_typ gsb_fn((i32, vint0) :: nil):: 
+               insn_call eid0 false attrs gse_typ gse_fn((i32, vint0) :: nil)::
+               insn_call fake_id true attrs dstk_typ dstk_fn nil::
+               (cs23' ++ cs24'))
+              tmn2' (updateAddAL _ lc2' i0 gr2) als2'):: ECs2)
+            gl2 fs2 M2''')).
+          eapply LLVMopsem.dsReturn; eauto.
+            unfold LLVMopsem.returnUpdateLocals. simpl.
+            rewrite J1. auto.
+
+        rewrite <- (@trace_app_nil__eq__trace trace_nil).
+        apply LLVMopsem.dsop_star_cons with (state2:=
+          (LLVMopsem.mkState S2 (los, nts) Ps2
+            ((LLVMopsem.mkEC (fdef_intro fh2' bs2') B2'
+              (insn_call eid0 false attrs gse_typ gse_fn((i32, vint0) :: nil)::
+               insn_call fake_id true attrs dstk_typ dstk_fn nil::
+               (cs23' ++ cs24'))
+              tmn2' (updateAddAL _ (updateAddAL _ lc2' i0 gr2) bid0 null) 
+              als2'):: ECs2)
+            gl2 fs2 M2''')).
+          eapply LLVMopsem.dsExCall with (fid:=gsb_fid)
+            (gvs:=(int2GV 0 :: nil))(oresult:=Some null); eauto.
+            eapply gsb_is_found; eauto. admit.
+
+        rewrite <- (@trace_app_nil__eq__trace trace_nil).
+        apply LLVMopsem.dsop_star_cons with (state2:=
+          (LLVMopsem.mkState S2 (los, nts) Ps2
+            ((LLVMopsem.mkEC (fdef_intro fh2' bs2') B2'
+              (insn_call fake_id true attrs dstk_typ dstk_fn nil:: 
+               cs23' ++ cs24')
+              tmn2' (updateAddAL _ (updateAddAL _ (updateAddAL _ lc2' i0 gr2) 
+                bid0 null) eid0 null) als2'):: ECs2)
+            gl2 fs2 M2''')); auto.
+          eapply LLVMopsem.dsExCall with (fid:=gse_fid)
+            (gvs:=(int2GV 0 :: nil))(oresult:=Some null); eauto.
+            eapply gse_is_found; eauto. admit.
+
+        rewrite <- (@trace_app_nil__eq__trace trace_nil).
+        apply LLVMopsem.dsop_star_cons with (state2:=
+          (LLVMopsem.mkState S2 (los, nts) Ps2
+            ((LLVMopsem.mkEC (fdef_intro fh2' bs2') B2'
+              (cs23' ++ cs24')
+              tmn2' (updateAddAL _ (updateAddAL _ (updateAddAL _ lc2' i0 gr2) 
+                bid0 null) eid0 null) als2'):: ECs2)
+            gl2 fs2 M2''')); auto.
+          eapply LLVMopsem.dsExCall; simpl; eauto.
+            eapply dstk_is_found; eauto.
+            eapply dstk_spec; eauto.
+
+      split; auto using inject_incr_refl.
+      SSSSCase "sim".
+      repeat (split; auto).
+          eapply cmds_at_block_tail_next; eauto.
+
+          destruct Heqb2' as [l2' [ps2' [cs21' Heqb2']]]; subst.
+          exists l2'. exists ps2'. exists (cs21' ++
+              [insn_call i0 false c t (wrap_call v) p] ++
+              [insn_call bid0 false attrs gsb_typ gsb_fn [(i32, vint0)]] ++
+              [insn_call eid0 false attrs gse_typ gse_fn [(i32, vint0)]] ++
+              [insn_call fake_id true attrs dstk_typ dstk_fn nil]). 
+          simpl_env. auto.
+ 
+          exists ex_ids'. exists rm2'.
+          exists ex_ids3'. exists ex_ids4'. exists cs23'. exists cs24'.
+          repeat (split; auto).    
+            clear - J2 Hrsim' HeqR. admit.
+            clear - J2 Hrsim' HeqR. admit.
+
+    SSCase "ct isnt ptr".
+      inv Hcall'.
+      simpl in Httmn.
+      destruct (isPointerTypB RetTy).
+    SSSCase "rt is ptr". 
+      inv H1.
+      remember (SBopsem.get_reg_metadata (los, nts) gl2 rm Result) as oRmd.
+      destruct oRmd as [[bgv1 egv1]|]; inv HeqRet.
+      assert (exists bv2, exists ev2, exists bgv2, exists egv2,
+        get_reg_metadata rm2 Result = Some (bv2, ev2) /\
+        getOperandValue (los,nts) bv2 lc2 gl2 = Some bgv2 /\
+        getOperandValue (los,nts) ev2 lc2 gl2 = Some egv2 /\
+        gv_inject mi bgv1 bgv2 /\
+        gv_inject mi egv1 egv2) as J.
+        clear - HeqoRmd Hrsim. 
+        destruct Hrsim as [_ Hrsim].
+        apply Hrsim; auto.
+      destruct J as [bv2 [ev2 [bgv2 [egv2 [Hgetrmd [Hgetbgv2 [Hgetegv2 [Hinj1 
+        Hinj2]]]]]]]]. rewrite Hgetrmd in Httmn. inv Httmn.
+      destruct (@stk_ret_sim (los,nts) Mem0 M2 mi mgb MM bgv2 egv2) as 
+        [M2' [M2'' [Hsbase [Hsbound [Hmsim3 [Hwfmi3 [Hgbase Hgbound]]]]]]]; 
+        auto.
+      eapply free_allocas_sim in Hmsim3; eauto.
+      destruct Hmsim3 as [M2''' [Hfree2' [Hmsim2' Hwfmi2']]].
+      symmetry in Heqogr.
+      eapply simulation__getOperandValue in Heqogr; eauto.
+      destruct Heqogr as [gr2 [J1 J2]]. 
+      exists (LLVMopsem.mkState S2 (los, nts) Ps2
+        ((LLVMopsem.mkEC (fdef_intro fh2' bs2') B2'
+            (cs23' ++ cs24') tmn2' (updateAddAL _ lc2' i0 gr2)
+            als2'):: ECs2)
+        gl2 fs2 M2''').
+      exists mi.
+      split.
+      SSSSCase "dsop_star".
+        rewrite <- (@trace_app_nil__eq__trace trace_nil).
+        apply LLVMopsem.dsop_star_cons with (state2:=
+          (LLVMopsem.mkState S2 (los, nts) Ps2
+            ((LLVMopsem.mkEC (fdef_intro fh2 bs2) B2
+              ((insn_call fake_id true attrs sse_typ sse_fn 
+                  ((p8, ev2)::(i32, vint0) :: nil))::nil)
+              (insn_return rid RetTy Result) lc2 als2)::
+             (LLVMopsem.mkEC (fdef_intro fh2' bs2') B2'
+              ((insn_call i0 false c t (wrap_call v) p)::
+               (insn_call fake_id true attrs dstk_typ dstk_fn nil)::
+               cs23' ++ cs24')
+              tmn2' lc2' als2'):: ECs2)
+            gl2 fs2 M2')). 
+          eapply LLVMopsem.dsExCall with (fid:=ssb_fid)
+            (gvs:=(bgv2 :: int2GV 0 :: nil))(oresult:=None); eauto.
+            eapply ssb_is_found; eauto.
+            simpl. rewrite Hgetbgv2. auto.
+
+        rewrite <- (@trace_app_nil__eq__trace trace_nil).
+        apply LLVMopsem.dsop_star_cons with (state2:=
+          (LLVMopsem.mkState S2 (los, nts) Ps2
+            ((LLVMopsem.mkEC (fdef_intro fh2 bs2) B2 nil
+              (insn_return rid RetTy Result) lc2 als2)::
+             (LLVMopsem.mkEC (fdef_intro fh2' bs2') B2'
+              ((insn_call i0 false c t (wrap_call v) p)::
+               (insn_call fake_id true attrs dstk_typ dstk_fn nil)::
+              (cs23' ++ cs24'))
+              tmn2' lc2' als2'):: ECs2)
+            gl2 fs2 M2'')).
+          eapply LLVMopsem.dsExCall with (fid:=sse_fid)
+            (gvs:=(egv2 :: int2GV 0 :: nil))(oresult:=None); eauto.
+            eapply sse_is_found; eauto.
+            simpl. rewrite Hgetegv2. auto.
+
+        rewrite <- (@trace_app_nil__eq__trace trace_nil).
+        apply LLVMopsem.dsop_star_cons with (state2:=
+          (LLVMopsem.mkState S2 (los, nts) Ps2
+            ((LLVMopsem.mkEC (fdef_intro fh2' bs2') B2'
+               (insn_call fake_id true attrs dstk_typ dstk_fn nil::
+                (cs23' ++ cs24'))
+              tmn2' (updateAddAL _ lc2' i0 gr2) als2'):: ECs2)
+            gl2 fs2 M2''')).
+          eapply LLVMopsem.dsReturn; eauto.
+            unfold LLVMopsem.returnUpdateLocals. simpl.
+            rewrite J1. auto.
+
+        rewrite <- (@trace_app_nil__eq__trace trace_nil).
+        apply LLVMopsem.dsop_star_cons with (state2:=
+          (LLVMopsem.mkState S2 (los, nts) Ps2
+            ((LLVMopsem.mkEC (fdef_intro fh2' bs2') B2'
+              (cs23' ++ cs24')
+              tmn2' (updateAddAL _ lc2' i0 gr2) als2'):: ECs2)
+            gl2 fs2 M2''')); auto.
+          eapply LLVMopsem.dsExCall; simpl; eauto.
+            eapply dstk_is_found; eauto.
+            eapply dstk_spec; eauto.
+
+      split; auto using inject_incr_refl.
+      SSSSCase "sim".
+      repeat (split; auto).
+          eapply cmds_at_block_tail_next; eauto.
+
+          destruct Heqb2' as [l2' [ps2' [cs21' Heqb2']]]; subst.
+          exists l2'. exists ps2'. exists (cs21' ++
+              [insn_call i0 false c t (wrap_call v) p] ++
+              [insn_call fake_id true attrs dstk_typ dstk_fn nil]). 
+          simpl_env. auto.
+ 
+          exists ex_ids'. exists rm2'.
+          exists ex_ids3'. exists ex_ids4'. exists cs23'. exists cs24'.
+          apply reg_simulation__updateAddAL_lc with (i0:=i0)(gv:=ogr)(gv':=gr2) 
+            in Hrsim'; auto.
+            repeat (split; auto).    
+            admit. admit.
+
+    SSSCase "rt isnt ptr". 
+      inv H1. inv HeqRet. inv Httmn.
+      destruct (@stk_ret_sim (los,nts) Mem0 M2 mi mgb MM null null) as 
+        [M2' [M2'' [Hsbase [Hsbound [Hmsim3 [Hwfmi3 [Hgbase Hgbound]]]]]]]; 
+        auto.
+      eapply free_allocas_sim in Hmsim3; eauto.
+      destruct Hmsim3 as [M2''' [Hfree2' [Hmsim2' Hwfmi2']]].
+      symmetry in Heqogr.
+      eapply simulation__getOperandValue in Heqogr; eauto.
+      destruct Heqogr as [gr2 [J1 J2]]. 
+      exists (LLVMopsem.mkState S2 (los, nts) Ps2
+        ((LLVMopsem.mkEC (fdef_intro fh2' bs2') B2'
+            (cs23' ++ cs24') tmn2' (updateAddAL _ lc2' i0 gr2)
+            als2'):: ECs2)
+        gl2 fs2 M2''').
+      exists mi.
+      split.
+      SSSSCase "dsop_star".
+        rewrite <- (@trace_app_nil__eq__trace trace_nil).
+        apply LLVMopsem.dsop_star_cons with (state2:=
+          (LLVMopsem.mkState S2 (los, nts) Ps2
+            ((LLVMopsem.mkEC (fdef_intro fh2 bs2) B2
+              ((insn_call fake_id true attrs sse_typ sse_fn 
+                  ((p8, vnullp8)::(i32, vint0) :: nil))::nil)
+              (insn_return rid RetTy Result) lc2 als2)::
+             (LLVMopsem.mkEC (fdef_intro fh2' bs2') B2'
+              ((insn_call i0 false c t (wrap_call v) p)::
+               (insn_call fake_id true attrs dstk_typ dstk_fn nil)::
+               cs23' ++ cs24')
+              tmn2' lc2' als2'):: ECs2)
+            gl2 fs2 M2')). 
+          eapply LLVMopsem.dsExCall with (fid:=ssb_fid)
+            (gvs:=(null :: int2GV 0 :: nil))(oresult:=None); eauto.
+            eapply ssb_is_found; eauto.
+
+        rewrite <- (@trace_app_nil__eq__trace trace_nil).
+        apply LLVMopsem.dsop_star_cons with (state2:=
+          (LLVMopsem.mkState S2 (los, nts) Ps2
+            ((LLVMopsem.mkEC (fdef_intro fh2 bs2) B2 nil
+              (insn_return rid RetTy Result) lc2 als2)::
+             (LLVMopsem.mkEC (fdef_intro fh2' bs2') B2'
+              ((insn_call i0 false c t (wrap_call v) p)::
+               (insn_call fake_id true attrs dstk_typ dstk_fn nil)::
+              (cs23' ++ cs24'))
+              tmn2' lc2' als2'):: ECs2)
+            gl2 fs2 M2'')).
+          eapply LLVMopsem.dsExCall with (fid:=sse_fid)
+            (gvs:=(null :: int2GV 0 :: nil))(oresult:=None); eauto.
+            eapply sse_is_found; eauto.
+
+        rewrite <- (@trace_app_nil__eq__trace trace_nil).
+        apply LLVMopsem.dsop_star_cons with (state2:=
+          (LLVMopsem.mkState S2 (los, nts) Ps2
+            ((LLVMopsem.mkEC (fdef_intro fh2' bs2') B2'
+              (insn_call fake_id true attrs dstk_typ dstk_fn nil::
+               (cs23' ++ cs24'))
+              tmn2' (updateAddAL _ lc2' i0 gr2) als2'):: ECs2)
+            gl2 fs2 M2''')).
+          eapply LLVMopsem.dsReturn; eauto.
+            unfold LLVMopsem.returnUpdateLocals. simpl.
+            rewrite J1. auto.
+
+        rewrite <- (@trace_app_nil__eq__trace trace_nil).
+        apply LLVMopsem.dsop_star_cons with (state2:=
+          (LLVMopsem.mkState S2 (los, nts) Ps2
+            ((LLVMopsem.mkEC (fdef_intro fh2' bs2') B2'
+              (cs23' ++ cs24')
+              tmn2' (updateAddAL _ lc2' i0 gr2) als2'):: ECs2)
+            gl2 fs2 M2''')); auto.
+          eapply LLVMopsem.dsExCall; simpl; eauto.
+            eapply dstk_is_found; eauto.
+            eapply dstk_spec; eauto.
+
+      split; auto using inject_incr_refl.
+      SSSSCase "sim".
+      repeat (split; auto).
+          eapply cmds_at_block_tail_next; eauto.
+
+          destruct Heqb2' as [l2' [ps2' [cs21' Heqb2']]]; subst.
+          exists l2'. exists ps2'. exists (cs21' ++
+              [insn_call i0 false c t (wrap_call v) p] ++
+              [insn_call fake_id true attrs dstk_typ dstk_fn nil]). 
+          simpl_env. auto.
+ 
+          exists ex_ids'. exists rm2'.
+          exists ex_ids3'. exists ex_ids4'. exists cs23'. exists cs24'.
+          apply reg_simulation__updateAddAL_lc with (i0:=i0)(gv:=ogr)(gv':=gr2) 
+            in Hrsim'; auto.
+            repeat (split; auto).    
+            admit. admit.
+Qed.
+
+Lemma SBpass_is_correct__dsReturnVoid : forall
+  (mi : meminj) (mgb : Values.block) (St : LLVMopsem.State) (S : system)
+  (TD : TargetData) (Ps : list product) (F : fdef) (B : block)
+  (rid : id) (lc : GVMap) (rm : SBopsem.rmetadata) (gl : GVMap)
+  (fs : GVMap) (F' : fdef) (B' : block) (c' : cmd) (tmn' : terminator)
+  (lc' : GVMap) (rm' : SBopsem.rmetadata) (EC : list SBopsem.ExecutionContext)
+  (cs' : list cmd) (Mem : mem) (MM : SBopsem.mmetadata) (als : list mblock)
+  (als' : list mblock)
+  (Hsim : sbState_simulates_State mi mgb
+           {|
+           SBopsem.CurSystem := S;
+           SBopsem.CurTargetData := TD;
+           SBopsem.CurProducts := Ps;
+           SBopsem.ECS := {|
+                          SBopsem.CurFunction := F;
+                          SBopsem.CurBB := B;
+                          SBopsem.CurCmds := nil;
+                          SBopsem.Terminator := insn_return_void rid;
+                          SBopsem.Locals := lc;
+                          SBopsem.Rmap := rm;
+                          SBopsem.Allocas := als |}
+                          :: {|
+                             SBopsem.CurFunction := F';
+                             SBopsem.CurBB := B';
+                             SBopsem.CurCmds := c' :: cs';
+                             SBopsem.Terminator := tmn';
+                             SBopsem.Locals := lc';
+                             SBopsem.Rmap := rm';
+                             SBopsem.Allocas := als' |} :: EC;
+           SBopsem.Globals := gl;
+           SBopsem.FunTable := fs;
+           SBopsem.Mem := Mem;
+           SBopsem.Mmap := MM |} St)
+  (Mem' : mem)
+  (H : Instruction.isCallInst c' = true)
+  (H0 : free_allocas TD Mem als = ret Mem')
+  (H1 : getCallerReturnID c' = merror),
+  exists St' : LLVMopsem.State,
+     exists mi' : meminj,
+       LLVMopsem.dsop_star St St' trace_nil /\
+       sbState_simulates_State mi' mgb
+         {|
+         SBopsem.CurSystem := S;
+         SBopsem.CurTargetData := TD;
+         SBopsem.CurProducts := Ps;
+         SBopsem.ECS := {|
+                        SBopsem.CurFunction := F';
+                        SBopsem.CurBB := B';
+                        SBopsem.CurCmds := cs';
+                        SBopsem.Terminator := tmn';
+                        SBopsem.Locals := lc';
+                        SBopsem.Rmap := rm';
+                        SBopsem.Allocas := als' |} :: EC;
+         SBopsem.Globals := gl;
+         SBopsem.FunTable := fs;
+         SBopsem.Mem := Mem';
+         SBopsem.Mmap := MM |} St' /\ inject_incr mi mi'.
+Proof. 
+  intros.
+  destruct_ctx_return.
+  inv Htcmds.
+  simpl in H1.
+  destruct n; inv H1.
+  unfold call_suffix in Hcall'. inv Hcall'.
+  inv Httmn.
+  eapply free_allocas_sim in HsimM; eauto.
+  destruct HsimM as [M2' [Hfree2' [Hmsim2' Hwfmi2']]].
+  exists (LLVMopsem.mkState S2 (los, nts) Ps2
+        ((LLVMopsem.mkEC (fdef_intro fh2' bs2') B2'
+            (cs23' ++ cs24') tmn2' lc2' als2'):: ECs2)
+        gl2 fs2 M2').
+  exists mi.
+  split.
+    SCase "dsop_star".
+      rewrite <- (@trace_app_nil__eq__trace trace_nil).
+      apply LLVMopsem.dsop_star_cons with (state2:=
+        (LLVMopsem.mkState S2 (los, nts) Ps2
+          ((LLVMopsem.mkEC (fdef_intro fh2' bs2') B2'
+            ((insn_call fake_id true attrs dstk_typ dstk_fn nil)::
+            (cs23' ++ cs24'))
+            tmn2' lc2' als2'):: ECs2)
+          gl2 fs2 M2')).
+        eapply LLVMopsem.dsReturnVoid; eauto.
+    
+      rewrite <- (@trace_app_nil__eq__trace trace_nil).
+      apply LLVMopsem.dsop_star_cons with (state2:=
+        (LLVMopsem.mkState S2 (los, nts) Ps2
+          ((LLVMopsem.mkEC (fdef_intro fh2' bs2') B2'
+            (cs23' ++ cs24')
+            tmn2' lc2' als2'):: ECs2)
+          gl2 fs2 M2')); auto.
+        eapply LLVMopsem.dsExCall; simpl; eauto.
+          eapply dstk_is_found; eauto.
+          eapply dstk_spec; eauto.
+    
+    split; auto using inject_incr_refl.
+    SSSCase "sim".
+    repeat (split; auto).
+        eapply cmds_at_block_tail_next; eauto.
+     
+        destruct Heqb2' as [l2' [ps2' [cs21' Heqb2']]]; subst.
+        exists l2'. exists ps2'. exists (cs21' ++
+            [insn_call i0 true c t (wrap_call v) p] ++
+            [insn_call fake_id true attrs dstk_typ dstk_fn nil]). 
+        simpl_env. auto.
+    
+        exists ex_ids'. exists rm2'.
+        exists ex_ids3'. exists ex_ids4'. exists cs23'. exists cs24'.
+        repeat (split; auto).
+Qed.
+
+Ltac destruct_ctx_other :=
+match goal with
+| [Hsim : sbState_simulates_State _ _
+           {|
+           SBopsem.CurSystem := _;
+           SBopsem.CurTargetData := ?TD;
+           SBopsem.CurProducts := _;
+           SBopsem.ECS := {|
+                          SBopsem.CurFunction := ?F;
+                          SBopsem.CurBB := _;
+                          SBopsem.CurCmds := ?c::_;
+                          SBopsem.Terminator := _;
+                          SBopsem.Locals := _;
+                          SBopsem.Rmap := _;
+                          SBopsem.Allocas := _ |} :: _;
+           SBopsem.Globals := _;
+           SBopsem.FunTable := _;
+           SBopsem.Mem := _;
+           SBopsem.Mmap := _ |} ?St |- _] =>
+  destruct St as [S2 TD2 Ps2 ECs2 gl2 fs2 M2];
+  destruct TD as [los nts];
+  destruct Hsim as [Hwfs [HMinS [Htsym [Heq1 [Htps [HsimECs [Heq2 [Heq3 
+    [Hwfg [Hwfmi HsimM]]]]]]]]]];
+    subst;
+  destruct ECs2 as [|[F2 B2 cs2 tmn2 lc2 als2] ECs2];
+    try solve [inversion HsimECs];
+  simpl in HsimECs;
+  destruct HsimECs as [HsimEC HsimECs];
+  destruct F as [fh1 bs1];
+  destruct F2 as [fh2 bs2];
+  destruct HsimEC as [HBinF [HFinPS [Htfdef [Heq0 [Hasim [Hnth [Heqb1 [Heqb2 
+    [ex_ids [rm2 [ex_ids3 [ex_ids4 [cs22 [cs23 [Hgenmeta [Hrsim [Hinc [Hfresh 
+    [Htcmds [Httmn Heq2]]]]]]]]]]]]]]]]]]]]; subst
+end.
+
+Lemma SBpass_is_correct__dsBop : forall (mi : meminj) (mgb : Values.block)
+  (St : LLVMopsem.State) (S : system) (TD : TargetData) (Ps : list product)
+  (F : fdef) (B : block) (lc : GVMap) (rm : SBopsem.rmetadata) (gl : GVMap)
+  (fs : GVMap) (id0 : id) (bop0 : bop) (sz0 : sz) (v1 : value) (v2 : value)
+  (EC : list SBopsem.ExecutionContext) (cs : list cmd) (tmn : terminator)
+  (Mem : mem) (MM : SBopsem.mmetadata) (als : list mblock)
+  (Hsim : sbState_simulates_State mi mgb
+           {|
+           SBopsem.CurSystem := S;
+           SBopsem.CurTargetData := TD;
+           SBopsem.CurProducts := Ps;
+           SBopsem.ECS := {|
+                          SBopsem.CurFunction := F;
+                          SBopsem.CurBB := B;
+                          SBopsem.CurCmds := insn_bop id0 bop0 sz0 v1 v2
+                                             :: cs;
+                          SBopsem.Terminator := tmn;
+                          SBopsem.Locals := lc;
+                          SBopsem.Rmap := rm;
+                          SBopsem.Allocas := als |} :: EC;
+           SBopsem.Globals := gl;
+           SBopsem.FunTable := fs;
+           SBopsem.Mem := Mem;
+           SBopsem.Mmap := MM |} St)
+  (gv3 : GenericValue)
+  (H : BOP TD lc gl bop0 sz0 v1 v2 = ret gv3),
+  exists St' : LLVMopsem.State,
+     exists mi' : meminj,
+       LLVMopsem.dsop_star St St' trace_nil /\
+       sbState_simulates_State mi' mgb
+         {|
+         SBopsem.CurSystem := S;
+         SBopsem.CurTargetData := TD;
+         SBopsem.CurProducts := Ps;
+         SBopsem.ECS := {|
+                        SBopsem.CurFunction := F;
+                        SBopsem.CurBB := B;
+                        SBopsem.CurCmds := cs;
+                        SBopsem.Terminator := tmn;
+                        SBopsem.Locals := updateAddAL GenericValue lc id0 gv3;
+                        SBopsem.Rmap := rm;
+                        SBopsem.Allocas := als |} :: EC;
+         SBopsem.Globals := gl;
+         SBopsem.FunTable := fs;
+         SBopsem.Mem := Mem;
+         SBopsem.Mmap := MM |} St' /\ inject_incr mi mi'.
+Proof.
+  intros.
+  destruct_ctx_other.
+  simpl in Htcmds.
+  remember (trans_cmds ex_ids3 rm2 cs) as R.
+  destruct R as [[ex_ids2 cs2]|]; inv Htcmds.
+  eapply simulation__BOP in H; eauto.
+  destruct H as [gv3' [Hbop Hinj]].
+  exists (LLVMopsem.mkState S2 (los, nts) Ps2
+          ((LLVMopsem.mkEC (fdef_intro fh2 bs2) B2
+            (cs2 ++ cs23) tmn2 (updateAddAL GenericValue lc2 id0 gv3') als2):: 
+            ECs2) gl2 fs2 M2).
+  exists mi.
+  split.
+    rewrite <- (@trace_app_nil__eq__trace trace_nil).
+    eapply LLVMopsem.dsop_star_cons; eauto.
+      apply LLVMopsem.dsBop; auto.
+
+    split; auto using inject_incr_refl.
+    repeat (split; auto).
+      eapply cmds_at_block_tail_next; eauto.
+      eapply cmds_at_block_tail_next; eauto.
+
+      exists ex_ids. exists rm2.
+      exists ex_ids3. exists ex_ids4. exists cs2. exists cs23.
+      simpl in Hfresh. destruct Hfresh as [Hfresh1 Hfresh2].
+      split; auto.
+      split.
+        clear - Hfresh1 Hrsim Hinj.
+        destruct Hfresh1 as [Hnotin _]. 
+        unfold getCmdIDs in Hnotin. simpl in Hnotin.
+        apply reg_simulation__updateAddAL_lc; try solve [auto | fsetdec].
+          admit.
+      repeat (split; auto).
+Qed.
+
+Lemma SBpass_is_correct__dsMalloc : forall (mi : meminj) (mgb : Values.block)
+  (St : LLVMopsem.State) (S : system) (TD : TargetData) (Ps : list product)
+  (F : fdef) (B : block) (lc : GVMap) (rm : AssocList SBopsem.metadata)
+  (gl : GVMap) (fs : GVMap) (id0 : atom) (t : typ) (v : value) (align0 : align)
+  (EC : list SBopsem.ExecutionContext) (cs : list cmd) (tmn : terminator)
+  (Mem : mem) (MM : SBopsem.mmetadata) (als : list mblock) 
+  (Hsim : sbState_simulates_State mi mgb
+           {|
+           SBopsem.CurSystem := S;
+           SBopsem.CurTargetData := TD;
+           SBopsem.CurProducts := Ps;
+           SBopsem.ECS := {|
+                          SBopsem.CurFunction := F;
+                          SBopsem.CurBB := B;
+                          SBopsem.CurCmds := insn_malloc id0 t v align0 :: cs;
+                          SBopsem.Terminator := tmn;
+                          SBopsem.Locals := lc;
+                          SBopsem.Rmap := rm;
+                          SBopsem.Allocas := als |} :: EC;
+           SBopsem.Globals := gl;
+           SBopsem.FunTable := fs;
+           SBopsem.Mem := Mem;
+           SBopsem.Mmap := MM |} St)
+  (gn : GenericValue) (Mem' : mem) (tsz : sz) (mb : mblock) (lc' : GVMap)
+  (rm' : SBopsem.rmetadata) (n : Z) (H : getTypeAllocSize TD t = ret tsz)
+  (H0 : getOperandValue TD v lc gl = ret gn) 
+  (H1 : malloc TD Mem tsz gn align0 = ret (Mem', mb))
+  (H2 : GV2int TD Size.ThirtyTwo gn = ret n)
+  (H3 : SBopsem.prop_reg_metadata lc rm id0 (blk2GV TD mb)
+         {|
+         SBopsem.md_base := SBopsem.base2GV TD mb;
+         SBopsem.md_bound := SBopsem.bound2GV TD mb tsz n |} = 
+       (lc', rm')),
+  exists St' : LLVMopsem.State,
+     exists mi' : meminj,
+       LLVMopsem.dsop_star St St' trace_nil /\
+       sbState_simulates_State mi' mgb
+         {|
+         SBopsem.CurSystem := S;
+         SBopsem.CurTargetData := TD;
+         SBopsem.CurProducts := Ps;
+         SBopsem.ECS := {|
+                        SBopsem.CurFunction := F;
+                        SBopsem.CurBB := B;
+                        SBopsem.CurCmds := cs;
+                        SBopsem.Terminator := tmn;
+                        SBopsem.Locals := lc';
+                        SBopsem.Rmap := rm';
+                        SBopsem.Allocas := als |} :: EC;
+         SBopsem.Globals := gl;
+         SBopsem.FunTable := fs;
+         SBopsem.Mem := Mem';
+         SBopsem.Mmap := MM |} St' /\ inject_incr mi mi'.
+Proof.
+  intros.
+  destruct_ctx_other.
+  simpl in Hfresh. destruct Hfresh as [Hnotin Hfresh].
+  apply trans_cmds_inv in Htcmds.
+  destruct Htcmds as [ex_ids5 [cs1' [cs2' [Htcmd [Htcmds Heq]]]]]; subst.
+  simpl in Htcmd.
+  remember (lookupAL (id * id) rm2 id0) as R1.
+  destruct R1 as [[bid eid]|]; try solve [inversion Htcmd].
+  remember (mk_tmp ex_ids3) as R2.
+  destruct R2 as [tmp ex_ids6].
+  inv Htcmd.
+  invert_prop_reg_metadata.
+  assert (Hmalloc:=H1).
+  apply mem_simulation__malloc with (MM:=MM)(mgb:=mgb)(Mem2:=M2)(mi:=mi) in H1;
+    auto.
+  destruct H1 as [mi' [Mem2' [mb' [H11 [H16 [H12 [H13 [H14 H15]]]]]]]].
+  simpl.
+  exists (LLVMopsem.mkState S2 (los, nts) Ps2
+          ((LLVMopsem.mkEC (fdef_intro fh2 bs2) B2
+            (cs2' ++ cs23) tmn2 
+                (updateAddAL _ 
+                  (updateAddAL _ 
+                    (updateAddAL _ 
+                      (updateAddAL GenericValue lc2 id0 (blk2GV (los, nts) mb'))
+                      tmp (SBopsem.bound2GV (los, nts) mb' tsz n))
+                    bid (SBopsem.base2GV (los, nts) mb'))
+                  eid (SBopsem.bound2GV (los, nts) mb' tsz n))
+             als2):: 
+            ECs2) gl2 fs2 Mem2').
+  exists mi'.
+  split.
+  SCase "opsem".
+    rewrite <- (@trace_app_nil__eq__trace trace_nil).
+    apply LLVMopsem.dsop_star_cons with (state2:=
+        LLVMopsem.mkState S2 (los, nts) Ps2
+          ((LLVMopsem.mkEC (fdef_intro fh2 bs2) B2
+             (insn_gep tmp false t (value_id id0) 
+                (Cons_list_value v Nil_list_value):: 
+              insn_cast bid castop_bitcast (typ_pointer t)(value_id id0) p8 :: 
+              insn_cast eid castop_bitcast (typ_pointer t)(value_id tmp) p8 :: 
+              cs2' ++ cs23)
+             tmn2 
+             (updateAddAL GenericValue lc2 id0 (blk2GV (los, nts) mb'))
+             als2):: 
+            ECs2) gl2 fs2 Mem2'); auto.
+      eapply simulation__getOperandValue with (mi:=mi)(Mem2:=M2) in H0; eauto.
+      destruct H0 as [gn' [H00 H01]].
+      unfold malloc in H11.
+      erewrite simulation__eq__GV2int in H11; eauto.
+
+    rewrite <- (@trace_app_nil__eq__trace trace_nil).
+    apply LLVMopsem.dsop_star_cons with (state2:=
+        LLVMopsem.mkState S2 (los, nts) Ps2
+          ((LLVMopsem.mkEC (fdef_intro fh2 bs2) B2
+             (insn_cast bid castop_bitcast (typ_pointer t)(value_id id0) p8 :: 
+              insn_cast eid castop_bitcast (typ_pointer t)(value_id tmp) p8 :: 
+              cs2' ++ cs23)
+             tmn2 
+             (updateAddAL _
+               (updateAddAL GenericValue lc2 id0 (blk2GV (los,nts) mb'))
+               tmp (SBopsem.bound2GV (los,nts) mb' tsz n))
+             als2):: 
+            ECs2) gl2 fs2 Mem2'); auto.
+      assert (exists gn', getOperandValue (los,nts) v lc2 gl2 = ret gn' /\
+          GV2int (los,nts) Size.ThirtyTwo gn = 
+          GV2int (los,nts) Size.ThirtyTwo gn') as H4.
+        eapply simulation__getOperandValue with (Mem2:=M2) in H0; eauto.
+        destruct H0 as [gv' [H00 H01]].
+        exists gv'. split; auto.
+          rewrite simulation__eq__GV2int with (mi:=mi)(gn':=gv'); eauto.
+      destruct H4 as [gn' [H41 H42]].
+      apply LLVMopsem.dsGEP with (mp:=blk2GV (los,nts) mb')(vidxs:=[gn']); auto.
+        simpl.
+        rewrite lookupAL_updateAddAL_eq; auto.
+
+        simpl.
+        assert(getOperandValue (los,nts) v
+          (updateAddAL _ lc2 id0 (blk2GV (los,nts) mb')) gl2 = 
+          getOperandValue (los,nts) v lc2 gl2) as EQ'.
+          clear - Hnotin HeqR1. 
+          destruct Hnotin as [Hnotin1 [Hnotin2 _ ]]. simpl in Hnotin2.
+
+          rewrite <- getOperandValue_eq_fresh_id; auto.
+            unfold getCmdIDs in Hnotin1. simpl in Hnotin1.
+            eapply notin_codom__neq' in HeqR1; eauto.
+              destruct v; simpl in *; fsetdec.
+
+        rewrite EQ'. clear EQ'.
+        rewrite H41. auto.
+
+        unfold SBopsem.bound2GV, GEP, blk2GV, GV2ptr, ptr2GV, val2GV.
+        simpl.
+        rewrite <- H42. rewrite H2.
+        unfold Constant.typ2utyp.
+        assert (exists ut, 
+          Constant.typ2utyp_aux (Constant.subst_nts_by_nts nts nts) 
+            (typ_array 0%nat t) = Some (typ_array 0%nat ut) /\
+          getTypeAllocSize (los, nts) ut = getTypeAllocSize (los, nts) t) as EQ1.
+          destruct Heqb1 as [l1 [ps1 [cs11 Heqb1]]]; subst.
+          eapply wf_system__wf_cmd with (c:=insn_malloc id0 t v align0) in HBinF;
+            eauto.
+            inv HBinF. inv H21. 
+            (* ssa_static should check this typ is Constant.unifiable_typ
+               like wf_const_gid *)
+            admit.
+
+            apply in_or_app. simpl. auto.
+        destruct EQ1 as [ut [EQ1 EQ2]].
+        rewrite EQ1. simpl.
+        rewrite EQ2. rewrite H. simpl.
+        rewrite Int.add_commut.
+        rewrite Int.add_zero. auto.
+
+    rewrite <- (@trace_app_nil__eq__trace trace_nil).
+    apply LLVMopsem.dsop_star_cons with (state2:=
+        LLVMopsem.mkState S2 (los, nts) Ps2
+          ((LLVMopsem.mkEC (fdef_intro fh2 bs2) B2
+             (insn_cast eid castop_bitcast (typ_pointer t)(value_id tmp) p8 :: 
+              cs2' ++ cs23)
+             tmn2 
+             (updateAddAL _
+               (updateAddAL _
+                 (updateAddAL GenericValue lc2 id0 (blk2GV (los,nts) mb'))
+                 tmp (SBopsem.bound2GV (los,nts) mb' tsz n))
+               bid (SBopsem.base2GV (los,nts) mb'))               
+             als2):: 
+            ECs2) gl2 fs2 Mem2'); auto.
+      apply LLVMopsem.dsCast; auto.
+        unfold CAST. simpl.
+        rewrite <- lookupAL_updateAddAL_neq.
+          rewrite lookupAL_updateAddAL_eq.
+          auto.
+
+          clear - Hnotin HeqR1 HeqR2.
+          destruct Hnotin as [Hnotin1 [_ [Hnotin2 _]]]. 
+          unfold getCmdIDs in *. simpl in *.
+          eapply tmp_is_fresh; eauto. fsetdec.
+
+    rewrite <- (@trace_app_nil__eq__trace trace_nil).
+    apply LLVMopsem.dsop_star_cons with (state2:=
+       (LLVMopsem.mkState S2 (los, nts) Ps2
+          ((LLVMopsem.mkEC (fdef_intro fh2 bs2) B2
+            (cs2' ++ cs23) tmn2 
+                (updateAddAL _ 
+                  (updateAddAL _ 
+                    (updateAddAL _ 
+                      (updateAddAL GenericValue lc2 id0 (blk2GV (los, nts) mb'))
+                      tmp (SBopsem.bound2GV (los, nts) mb' tsz n))
+                    bid (SBopsem.base2GV (los, nts) mb'))                    
+                  eid (SBopsem.bound2GV (los, nts) mb' tsz n))
+             als2):: 
+            ECs2) gl2 fs2 Mem2')); auto.
+      apply LLVMopsem.dsCast; auto.
+        unfold CAST. simpl.
+        rewrite <- lookupAL_updateAddAL_neq.
+          rewrite lookupAL_updateAddAL_eq; auto.
+
+          destruct Hnotin as [Hnotin1 [Hnotin2 [Hnotin3 Hnotin4]]]. 
+          unfold getCmdIDs in *.
+          eapply tmp_is_fresh' with (tmp:=tmp) in HeqR1; eauto. 
+            destruct HeqR1; auto.
+            clear - Hnotin3. fsetdec.
+
+  split; auto.
+  split; auto.
+  split; auto.
+  split; auto.
+  split.
+  split.
+  split; auto.          
+  split; auto.          
+  split; auto.          
+  split; auto.          
+  split; auto.          
+  split; auto.          
+  split; auto.          
+  split; eauto using inject_incr__preserves__als_simulation.
+  split; auto.
+  split.
+    eapply cmds_at_block_tail_next; eauto.
+  split.
+    destruct Heqb2 as [l2 [ps2 [cs21 Heqb2]]]; subst.
+    exists l2. exists ps2. exists (cs21 ++
+                  (insn_malloc id0 t v align0
+                    :: insn_gep tmp false t (value_id id0)
+                         (Cons_list_value v Nil_list_value)
+                       :: insn_cast bid castop_bitcast 
+                            (typ_pointer t) (value_id id0) p8
+                          :: insn_cast eid castop_bitcast 
+                               (typ_pointer t) (value_id tmp) p8 :: nil)).
+    simpl_env. auto.
+  exists ex_ids. exists rm2.
+  exists ex_ids5. exists ex_ids4. exists cs2'. exists cs23.
+  split; auto.
+  split.
+  SCase "rsim".
+    eapply reg_simulation__updateAddAL_md; eauto.
+      eapply reg_simulation__updateAddAL_tmp; eauto.
+      eapply reg_simulation__updateAddAL_lc; eauto.
+        eapply inject_incr__preserves__reg_simulation; eauto.
+        admit.
+        admit.
+
+      unfold gv_inject, blk2GV, ptr2GV, val2GV.
+      simpl. apply val_cons_inject; eauto.
+
+      unfold gv_inject, SBopsem.base2GV, blk2GV, ptr2GV, val2GV.
+      simpl. clear - H14.
+      apply val_cons_inject; eauto.
+
+      unfold gv_inject, SBopsem.base2GV, blk2GV, ptr2GV, val2GV.
+      simpl. clear - H14.
+        apply val_cons_inject; eauto.
+          eapply val_inject_ptr; eauto.
+            rewrite Int.add_zero. auto.
+
+    split; auto.
+      clear - Hinc HeqR2. eapply mk_tmp_inc; eauto.
+    split; auto.
+      clear - Hinc HeqR2 Hfresh. eapply wf_freshs__mk_tmp; eauto.
+      
+      clear - HsimECs H13. 
+      eapply inject_incr__preserves__sbECs_simulate_ECs_tail; eauto.
+Qed.
+
+Lemma SBpass_is_correct__dsFree : forall (mi : meminj) (mgb : Values.block)
+  (St : LLVMopsem.State) (S : system) (TD : TargetData) (Ps : list product)
+  (F : fdef) (B : block) (lc : GVMap) (rm : rmetadata) (gl : GVMap)
+  (fs : GVMap) (fid : id) (t : typ) (v : value) (EC : list ExecutionContext)
+  (cs : list cmd) (tmn : terminator) (Mem0 : mem) (als : list mblock)
+  (MM : mmetadata)
+  (Hsim : sbState_simulates_State mi mgb
+           {|
+           CurSystem := S;
+           CurTargetData := TD;
+           CurProducts := Ps;
+           ECS := {|
+                  CurFunction := F;
+                  CurBB := B;
+                  CurCmds := insn_free fid t v :: cs;
+                  Terminator := tmn;
+                  Locals := lc;
+                  Rmap := rm;
+                  Allocas := als |} :: EC;
+           Globals := gl;
+           FunTable := fs;
+           Mem := Mem0;
+           Mmap := MM |} St)
+  (Mem' : mem)
+  (mptr0 : GenericValue)
+  (H : getOperandValue TD v lc gl = ret mptr0)
+  (H0 : free TD Mem0 mptr0 = ret Mem'),
+   exists St' : LLVMopsem.State,
+     exists mi' : meminj,
+       LLVMopsem.dsop_star St St' trace_nil /\
+       sbState_simulates_State mi' mgb
+         {|
+         CurSystem := S;
+         CurTargetData := TD;
+         CurProducts := Ps;
+         ECS := {|
+                CurFunction := F;
+                CurBB := B;
+                CurCmds := cs;
+                Terminator := tmn;
+                Locals := lc;
+                Rmap := rm;
+                Allocas := als |} :: EC;
+         Globals := gl;
+         FunTable := fs;
+         Mem := Mem';
+         Mmap := MM |} St' /\ inject_incr mi mi'.
+Proof.
+  intros.
+  destruct_ctx_other.
+  simpl in Hfresh. destruct Hfresh as [Hnotin Hfresh].
+  apply trans_cmds_inv in Htcmds.
+  destruct Htcmds as [ex_ids5 [cs1' [cs2' [Htcmd [Htcmds Heq]]]]]; subst.
+  simpl in Htcmd. 
+  inv Htcmd.
+  apply free_inv in H0.
+  destruct H0 as [blk [i0 [hi [lo [HeqR0 [J12 [HeqR2 H0]]]]]]].
+  eapply simulation__getOperandValue in H; eauto.
+  destruct H as [mptr0' [H1 H2]].
+  eapply simulation__GV2ptr in HeqR0; eauto.
+  destruct HeqR0 as [v' [J1 J2]].
+  inv J2.
+  eapply mem_simulation__free in H0; eauto.
+  destruct H0 as [Mem2' [Hfree2 [Hwfmi2  Hmsim2]]].
+  exists (LLVMopsem.mkState S2 (los, nts) Ps2
+          ((LLVMopsem.mkEC (fdef_intro fh2 bs2) B2
+            (cs2' ++ cs23) tmn2 lc2
+             als2):: 
+            ECs2) gl2 fs2 Mem2').
+  exists mi.
+  split.
+  SCase "opsem".
+    simpl.
+    rewrite <- (@trace_app_nil__eq__trace trace_nil).
+    eapply LLVMopsem.dsop_star_cons; eauto.
+      apply LLVMopsem.dsFree with (mptr:=mptr0'); auto.
+        unfold free.     
+        rewrite J1.
+        inversion_clear Hwfmi.
+        assert (H4':=H4).
+        apply mi_range_block in H4'. subst.
+        rewrite Int.add_zero.
+        destruct (zeq (Int.signed 31 i0) 0).
+          apply mi_bounds in H4.
+          rewrite <- H4. rewrite <- HeqR2.
+          assert (lo + 0 = lo) as EQ''. auto with zarith. 
+          rewrite EQ'' in Hfree2. clear EQ''.
+          assert (hi + 0 = hi) as EQ''. auto with zarith.
+          rewrite EQ'' in Hfree2. clear EQ''.
+          auto.
+
+          clear - J12 n. contradict J12; auto.          
+
+  repeat (split; auto).
+    eapply cmds_at_block_tail_next; eauto.
+
+    simpl_env in Heqb2. simpl in Heqb2.
+    eapply cmds_at_block_tail_next; eauto.
+
+  exists ex_ids. exists rm2.
+  exists ex_ids5. exists ex_ids4. exists cs2'. exists cs23.
+  split; auto.
+  split; auto.
+Qed.
+
+Lemma SBpass_is_correct__dsLoad_nptr : forall 
+  (mi : meminj) (mgb : Values.block) (St : LLVMopsem.State) (S : system)
+  (TD : TargetData) (Ps : list product) (F : fdef) (B : block) (lc : GVMap)
+  (rm : rmetadata) (gl : GVMap) (fs : GVMap) (id0 : id) (t : typ)
+  (align0 : align) (vp : value) (EC : list ExecutionContext) (cs : list cmd)
+  (tmn : terminator) (Mem0 : mem) (als : list mblock) (MM : mmetadata)
+  (Hsim : sbState_simulates_State mi mgb
+           {|
+           CurSystem := S;
+           CurTargetData := TD;
+           CurProducts := Ps;
+           ECS := {|
+                  CurFunction := F;
+                  CurBB := B;
+                  CurCmds := insn_load id0 t vp align0 :: cs;
+                  Terminator := tmn;
+                  Locals := lc;
+                  Rmap := rm;
+                  Allocas := als |} :: EC;
+           Globals := gl;
+           FunTable := fs;
+           Mem := Mem0;
+           Mmap := MM |} St)
+  (gvp : GenericValue) (gv : GenericValue) (md : metadata)
+  (H : SBopsem.get_reg_metadata TD gl rm vp = ret md)
+  (H0 : getOperandValue TD vp lc gl = ret gvp)
+  (H1 : assert_mptr TD t gvp md)
+  (H2 : mload TD Mem0 gvp t align0 = ret gv)
+  (H3 : isPointerTypB t = false),
+   exists St' : LLVMopsem.State,
+     exists mi' : meminj,
+       LLVMopsem.dsop_star St St' trace_nil /\
+       sbState_simulates_State mi' mgb
+         {|
+         CurSystem := S;
+         CurTargetData := TD;
+         CurProducts := Ps;
+         ECS := {|
+                CurFunction := F;
+                CurBB := B;
+                CurCmds := cs;
+                Terminator := tmn;
+                Locals := updateAddAL GenericValue lc id0 gv;
+                Rmap := rm;
+                Allocas := als |} :: EC;
+         Globals := gl;
+         FunTable := fs;
+         Mem := Mem0;
+         Mmap := MM |} St' /\ inject_incr mi mi'.
+Proof.
+  intros.
+  destruct_ctx_other.
+  simpl in Hfresh. destruct Hfresh as [Hnotin Hfresh].
+  apply trans_cmds_inv in Htcmds.
+  destruct Htcmds as [ex_ids5 [cs1' [cs2' [Htcmd [Htcmds Heq]]]]]; subst.
+  simpl in Htcmd. 
+  remember (get_reg_metadata rm2 vp) as R.
+  destruct R as [[bv ev]|]; try solve [inversion Htcmd].
+  remember (mk_tmp ex_ids3) as R1. 
+  destruct R1 as [ptmp ex_ids3'].
+  remember (isPointerTypB t) as R4.
+  destruct R4.
+  SCase "t is ptr".
+    unfold isPointerTyp in H3.
+    inv H3.
+
+  SCase "t isnt ptr".
+  inv Htcmd.
+  assert (J:=H1).
+  unfold SBopsem.assert_mptr in J.
+  destruct md as [md_base md_bound].
+  remember (GV2ptr (los,nts) (getPointerSize (los,nts)) gvp) as R.
+  destruct R; try solve [inversion J].
+  destruct v; try solve [inversion J].
+  remember (GV2ptr (los,nts) (getPointerSize (los,nts)) md_base) as R1.
+  destruct R1; try solve [inversion J].
+  destruct v; try solve [inversion J].
+  remember (GV2ptr (los,nts) (getPointerSize (los,nts)) md_bound) as R2.
+  destruct R2; try solve [inversion J].
+  destruct v; try solve [inversion J].
+  remember (getTypeAllocSize (los,nts) t) as R3.
+  destruct R3; try solve [inversion J].
+  eapply simulation__getOperandValue in H0; eauto.
+  destruct H0 as [gvp2 [H00 H01]].            
+  eapply simulation__mload in H2; eauto.
+  destruct H2 as [gv2 [H21 H22]].
+  assert (J':=Hrsim).
+  destruct J' as [Hrsim1 Hrsim2].
+  assert (HeqR8':=H).
+  apply Hrsim2 in HeqR8'.      
+  destruct HeqR8' as [bv2 [ev2 [bgv2 [egv2 [J1 [J2 [J3 [J4 J5]]]]]]]].
+  rewrite J1 in HeqR. inv HeqR.
+  exists (LLVMopsem.mkState S2 (los, nts) Ps2
+          ((LLVMopsem.mkEC (fdef_intro fh2 bs2) B2
+            (cs2' ++ cs23) tmn2 
+                  (updateAddAL _ 
+                    (updateAddAL GenericValue lc2 ptmp gvp2)
+                   id0 gv2)
+             als2):: 
+            ECs2) gl2 fs2 M2).
+  exists mi.
+  split.
+  SSCase "opsem".
+    simpl.
+    rewrite <- (@trace_app_nil__eq__trace trace_nil).
+    apply LLVMopsem.dsop_star_cons with (state2:=
+       (LLVMopsem.mkState S2 (los, nts) Ps2
+          ((LLVMopsem.mkEC (fdef_intro fh2 bs2) B2
+            (insn_call fake_id true attrs assert_typ assert_fn
+              ((p8, bv2)::(p8, ev2)::(p8, value_id ptmp)::(i32, type_size t):: 
+                 (i32, vint1) :: nil):: 
+             insn_load id0 t vp align0 :: cs2' ++ cs23) tmn2 
+            (updateAddAL GenericValue lc2 ptmp gvp2)
+             als2):: 
+            ECs2) gl2 fs2 M2)).
+      apply LLVMopsem.dsCast; auto.
+        unfold CAST. simpl. simpl in H00.
+        rewrite H00. auto.
+
+    rewrite <- (@trace_app_nil__eq__trace trace_nil).
+    apply LLVMopsem.dsop_star_cons with (state2:=
+       (LLVMopsem.mkState S2 (los, nts) Ps2
+          ((LLVMopsem.mkEC (fdef_intro fh2 bs2) B2
+            (insn_load id0 t vp align0 :: cs2' ++ cs23) tmn2 
+            (updateAddAL GenericValue lc2 ptmp gvp2)
+             als2):: 
+            ECs2) gl2 fs2 M2)).
+       clear - H00 J2 J3 J4 J5 J H00 H01 HeqR0 HeqR2 HeqR3 HeqR5.
+       eapply assert_mptr_fn__ok with (b:=b)(b0:=b0)(b1:=b1); eauto.
+
+    rewrite <- (@trace_app_nil__eq__trace trace_nil).
+    apply LLVMopsem.dsop_star_cons with (state2:=
+       (LLVMopsem.mkState S2 (los, nts) Ps2
+          ((LLVMopsem.mkEC (fdef_intro fh2 bs2) B2
+            (cs2' ++ cs23) tmn2 
+            (updateAddAL _ (updateAddAL GenericValue lc2 ptmp gvp2) id0 gv2)
+             als2):: 
+            ECs2) gl2 fs2 M2)); auto.
+      apply LLVMopsem.dsLoad with (mp:=gvp2); auto.
+        clear - J1 Hnotin HeqR1 HeqR2 HeqR3 H00.
+        destruct Hnotin as [Hnotin1 [_ [Hnotin2 _]]].
+        unfold getCmdIDs in *. simpl in *.
+        rewrite <- getOperandValue_eq_fresh_id; auto.
+          eapply get_reg_metadata_fresh' with (rm2:=rm2); eauto; try fsetdec.
+
+  repeat (split; auto).
+    eapply cmds_at_block_tail_next; eauto.
+
+    destruct Heqb2 as [l2 [ps2 [cs21 Heqb2]]]; subst.
+    exists l2. exists ps2. exists (cs21 ++
+                  (insn_cast ptmp castop_bitcast (typ_pointer t) vp p8
+                    :: insn_call fake_id true attrs assert_typ assert_fn
+                         ((p8, bv2)
+                          :: (p8, ev2)
+                             :: (p8, value_id ptmp)
+                                :: (i32, type_size t) :: (i32, vint1) :: nil)
+                       :: insn_load id0 t vp align0 :: nil)).
+    simpl_env. auto.
+
+  exists ex_ids. exists rm2.
+  exists ex_ids5. exists ex_ids4. exists cs2'. exists cs23.
+  split; auto.
+  split.
+    eapply reg_simulation__updateAddAL_lc; eauto.
+      eapply reg_simulation__updateAddAL_tmp; eauto.
+      admit.
+      admit.
+
+    split; auto.
+      clear - Hinc HeqR1. eapply mk_tmp_inc; eauto.
+    split; auto.
+      clear - Hinc HeqR1 Hfresh. eapply wf_freshs__mk_tmp; eauto.
+Qed.
+
+Lemma SBpass_is_correct__dsLoad_ptr : forall 
+  (mi : meminj) (mgb : Values.block) (St : LLVMopsem.State) (S : system)
+  (TD : TargetData) (Ps : list product) (F : fdef) (B : block) (lc : GVMap)
+  (rm : rmetadata) (gl : GVMap) (fs : GVMap) (id0 : id) (t : typ)
+  (align0 : align) (vp : value) (EC : list ExecutionContext) (cs : list cmd)
+  (tmn : terminator) (Mem0 : mem) (als : list mblock) (MM : mmetadata)
+  (Hsim : sbState_simulates_State mi mgb
+           {|
+           CurSystem := S;
+           CurTargetData := TD;
+           CurProducts := Ps;
+           ECS := {|
+                  CurFunction := F;
+                  CurBB := B;
+                  CurCmds := insn_load id0 t vp align0 :: cs;
+                  Terminator := tmn;
+                  Locals := lc;
+                  Rmap := rm;
+                  Allocas := als |} :: EC;
+           Globals := gl;
+           FunTable := fs;
+           Mem := Mem0;
+           Mmap := MM |} St)
+  md' lc' rm'
+  (gvp : GenericValue) (gv : GenericValue) (md : metadata)
+  (H : SBopsem.get_reg_metadata TD gl rm vp = ret md)
+  (H0 : getOperandValue TD vp lc gl = ret gvp)
+  (H1 : assert_mptr TD t gvp md)
+  (H2 : mload TD Mem0 gvp t align0 = ret gv)
+  (H3 : isPointerTypB t = true)
+  (H4 : get_mem_metadata TD MM gvp = md')
+  (H5 : prop_reg_metadata lc rm id0 gv md' = (lc', rm')),
+   exists St' : LLVMopsem.State,
+     exists mi' : meminj,
+       LLVMopsem.dsop_star St St' trace_nil /\
+       sbState_simulates_State mi' mgb
+         {|
+         CurSystem := S;
+         CurTargetData := TD;
+         CurProducts := Ps;
+         ECS := {|
+                CurFunction := F;
+                CurBB := B;
+                CurCmds := cs;
+                Terminator := tmn;
+                Locals := lc';
+                Rmap := rm';
+                Allocas := als |} :: EC;
+         Globals := gl;
+         FunTable := fs;
+         Mem := Mem0;
+         Mmap := MM |} St' /\ inject_incr mi mi'.
+Proof.
+  intros.
+  destruct_ctx_other.
+  simpl in Hfresh. destruct Hfresh as [Hnotin Hfresh].
+  apply trans_cmds_inv in Htcmds.
+  destruct Htcmds as [ex_ids5 [cs1' [cs2' [Htcmd [Htcmds Heq]]]]]; subst.
+  simpl in Htcmd. 
+  remember (get_reg_metadata rm2 vp) as R.
+  destruct R as [[bv ev]|]; try solve [inversion Htcmd].
+  remember (mk_tmp ex_ids3) as R1. 
+  destruct R1 as [ptmp ex_ids3'].
+  remember (isPointerTypB t) as R4.
+  destruct R4; try solve [inv H3].
+  remember (lookupAL (id * id) rm2 id0) as R5.
+  destruct R5 as [[bid0 eid0]|]; inv Htcmd.
+  assert (J:=H1).
+  unfold SBopsem.assert_mptr in J.
+  destruct md as [md_base md_bound].
+  remember (GV2ptr (los,nts) (getPointerSize (los,nts)) gvp) as R.
+  destruct R; try solve [inversion J].
+  destruct v; try solve [inversion J].
+  remember (GV2ptr (los,nts) (getPointerSize (los,nts)) md_base) as R1.
+  destruct R1; try solve [inversion J].
+  destruct v; try solve [inversion J].
+  remember (GV2ptr (los,nts) (getPointerSize (los,nts)) md_bound) as R2.
+  destruct R2; try solve [inversion J].
+  destruct v; try solve [inversion J].
+  remember (getTypeAllocSize (los,nts) t) as R3.
+  destruct R3; try solve [inversion J].
+  eapply simulation__getOperandValue in H0; eauto.
+  destruct H0 as [gvp2 [H00 H01]].            
+  unfold SBopsem.get_reg_metadata in H.
+  assert (H2':=H2).
+  eapply simulation__mload in H2'; eauto.
+  destruct H2' as [gv2 [H21 H22]].
+  assert (J':=Hrsim).
+  destruct J' as [Hrsim1 Hrsim2].
+  case_eq (SBopsem.get_mem_metadata (los,nts) MM gvp).
+  intros mb_base0 md_bound0 JJ.
+  assert (Hmsim':=HsimM).
+  destruct Hmsim' as [Hmsim1 [Hmgb [Hzeroout Hmsim2]]].
+  assert (JJ':=JJ).
+  assert (exists b, exists ofs, exists cm, gvp = (Vptr b ofs, cm)::nil) as EQ.
+    clear - H2.
+    eapply mload_inversion; eauto.
+  destruct EQ as [pb [pofs [cm EQ]]]. subst.
+  assert (getOperandValue (los, nts) (value_id ptmp) 
+      (updateAddAL _ (updateAddAL _ lc2 ptmp gvp2) id0 gv2) gl2 = ret gvp2) as K.
+    destruct Hnotin as [Hnotin1 [Hnotin2 [Hnotin3 Hnotin4]]]. 
+    simpl.
+    rewrite <- lookupAL_updateAddAL_neq; auto.
+      rewrite lookupAL_updateAddAL_eq; auto.
+      unfold getCmdIDs in Hnotin3. simpl in Hnotin3.
+      eapply tmp_is_fresh with (i0:=id0) in HeqR1; eauto. clear. fsetdec.
+
+  eapply Hmsim2 with (bid0:=bid0)(eid0:=eid0)(lc2:=
+    (updateAddAL _ (updateAddAL _ lc2 ptmp gvp2) id0 gv2)) in JJ'; eauto.
+  destruct JJ' as [bgv' [egv' [JJ1 [JJ2 JJ4]]]].
+  assert (HeqR9':=H).
+  apply Hrsim2 in HeqR9'.      
+  destruct HeqR9' as [bv2 [ev2 [bgv2 [egv2 [J1 [J2 [J3 [J4 J5]]]]]]]].
+  rewrite J1 in HeqR. inv HeqR.
+  exists (LLVMopsem.mkState S2 (los, nts) Ps2
+          ((LLVMopsem.mkEC (fdef_intro fh2 bs2) B2
+            (cs2' ++ cs23) tmn2 
+               (updateAddAL _ 
+                 (updateAddAL _ 
+                   (updateAddAL _ 
+                    (updateAddAL GenericValue lc2 ptmp gvp2)
+                   id0 gv2)
+                  bid0 bgv')
+                 eid0 egv')
+             als2):: 
+            ECs2) gl2 fs2 M2).
+  exists mi.
+  split.
+  SSCase "opsem".
+    simpl.
+    rewrite <- (@trace_app_nil__eq__trace trace_nil).
+    apply LLVMopsem.dsop_star_cons with (state2:=
+       (LLVMopsem.mkState S2 (los, nts) Ps2
+          ((LLVMopsem.mkEC (fdef_intro fh2 bs2) B2
+            (insn_call fake_id true attrs assert_typ assert_fn
+              ((p8, bv2)::(p8, ev2)::(p8, value_id ptmp)::(i32, type_size t):: 
+                 (i32, vint1) :: nil):: 
+             insn_load id0 t vp align0 :: 
+             insn_call bid0 false attrs gmb_typ gmb_fn
+               ((p8, value_id ptmp)::(p8, vnullp8)::(i32, vint1):: 
+                  (p32, vnullp32) :: nil) :: 
+             insn_call eid0 false attrs gme_typ gme_fn
+               ((p8, value_id ptmp)::(p8, vnullp8)::(i32, vint1):: 
+                  (p32, vnullp32) :: nil) :: 
+             cs2' ++ cs23) tmn2 
+            (updateAddAL GenericValue lc2 ptmp gvp2)
+             als2):: 
+            ECs2) gl2 fs2 M2)).
+      apply LLVMopsem.dsCast; auto.
+        unfold CAST. simpl. simpl in H00.
+        rewrite H00. auto.
+
+    rewrite <- (@trace_app_nil__eq__trace trace_nil).
+    apply LLVMopsem.dsop_star_cons with (state2:=
+       (LLVMopsem.mkState S2 (los, nts) Ps2
+          ((LLVMopsem.mkEC (fdef_intro fh2 bs2) B2
+            (insn_load id0 t vp align0 :: 
+             insn_call bid0 false attrs gmb_typ gmb_fn
+               ((p8, value_id ptmp)::(p8, vnullp8)::(i32, vint1):: 
+                  (p32, vnullp32) :: nil) :: 
+             insn_call eid0 false attrs gme_typ gme_fn
+               ((p8, value_id ptmp)::(p8, vnullp8)::(i32, vint1):: 
+                  (p32, vnullp32) :: nil) :: 
+             cs2' ++ cs23) tmn2 
+            (updateAddAL GenericValue lc2 ptmp gvp2)
+             als2):: 
+            ECs2) gl2 fs2 M2)).
+       clear - H00 J2 J3 J4 J5 J H00 H01 HeqR0 HeqR2 HeqR3 HeqR5 HeqR6.
+       eapply assert_mptr_fn__ok with (b:=b)(b0:=b0)(b1:=b1); eauto.
+
+    rewrite <- (@trace_app_nil__eq__trace trace_nil).
+    apply LLVMopsem.dsop_star_cons with (state2:=
+       (LLVMopsem.mkState S2 (los, nts) Ps2
+          ((LLVMopsem.mkEC (fdef_intro fh2 bs2) B2
+            (insn_call bid0 false attrs gmb_typ gmb_fn
+               ((p8, value_id ptmp)::(p8, vnullp8)::(i32, vint1):: 
+                  (p32, vnullp32) :: nil) :: 
+             insn_call eid0 false attrs gme_typ gme_fn
+               ((p8, value_id ptmp)::(p8, vnullp8)::(i32, vint1):: 
+                  (p32, vnullp32) :: nil) :: 
+             cs2' ++ cs23) tmn2 
+                 (updateAddAL _ (updateAddAL _ lc2 ptmp gvp2) id0 gv2)
+             als2):: 
+            ECs2) gl2 fs2 M2)); eauto.
+      apply LLVMopsem.dsLoad with (mp:=gvp2); auto.
+        clear - J1 Hnotin HeqR1 HeqR2 HeqR3 H00.
+        destruct Hnotin as [Hnotin1 [_ [Hnotin2 _]]].
+        unfold getCmdIDs in *. simpl in *.
+        rewrite <- getOperandValue_eq_fresh_id; auto.
+        eapply get_reg_metadata_fresh' with (rm2:=rm2); eauto; try fsetdec.
+
+  split; auto.
+  split; auto.
+  split; auto.
+  split; auto.
+  split; auto.
+  split; auto.
+  split; auto.
+  split; auto.
+  split; auto.
+  split; auto.
+  split; auto.
+  split; auto.
+  split; auto.
+  split; auto.
+  split.
+    eapply cmds_at_block_tail_next; eauto.
+  split.
+    destruct Heqb2 as [l2 [ps2 [cs21 Heqb2]]]; subst.
+    exists l2. exists ps2. exists (cs21 ++
+           (insn_cast ptmp castop_bitcast (typ_pointer t) vp p8 ::
+            insn_call fake_id true attrs assert_typ assert_fn
+              ((p8, bv2)::(p8, ev2)::(p8, value_id ptmp)::(i32, type_size t):: 
+                 (i32, vint1) :: nil):: 
+            insn_load id0 t vp align0 :: 
+            insn_call bid0 false attrs gmb_typ gmb_fn
+               ((p8, value_id ptmp)::(p8, vnullp8)::(i32, vint1):: 
+                  (p32, vnullp32) :: nil) :: 
+            insn_call eid0 false attrs gme_typ gme_fn
+               ((p8, value_id ptmp)::(p8, vnullp8)::(i32, vint1):: 
+                  (p32, vnullp32)::nil) :: nil)).
+    simpl_env. auto.
+  exists ex_ids. exists rm2.
+  exists ex_ids5. exists ex_ids4. exists cs2'. exists cs23.
+  split; auto.
+  split.
+    inv H5. rewrite JJ.
+    eapply reg_simulation__updateAddAL_prop; eauto.
+      eapply reg_simulation__updateAddAL_tmp; eauto.
+      admit.
+      admit.
+    split; auto.
+      clear - Hinc HeqR1. eapply mk_tmp_inc; eauto.
+    split; auto.
+      clear - Hinc HeqR1 Hfresh. eapply wf_freshs__mk_tmp; eauto.
+Qed.
+
+Lemma SBpass_is_correct__dsStore_nptr : forall 
+  (mi : meminj) (mgb : Values.block) (St : LLVMopsem.State) (S : system)
+  (TD : TargetData) (Ps : list product) (F : fdef) (B : block) (lc : GVMap)
+  (rm : rmetadata) (gl : GVMap) (fs : GVMap) (sid : id) (t : typ) 
+  (align0 : align) (v : value) (vp : value) (EC : list ExecutionContext)
+  (cs : list cmd) (tmn : terminator) (Mem0 : mem) (MM : mmetadata) 
+  (als : list mblock)
+  (Hsim : sbState_simulates_State mi mgb
+           {|
+           CurSystem := S;
+           CurTargetData := TD;
+           CurProducts := Ps;
+           ECS := {|
+                  CurFunction := F;
+                  CurBB := B;
+                  CurCmds := insn_store sid t v vp align0 :: cs;
+                  Terminator := tmn;
+                  Locals := lc;
+                  Rmap := rm;
+                  Allocas := als |} :: EC;
+           Globals := gl;
+           FunTable := fs;
+           Mem := Mem0;
+           Mmap := MM |} St)
+  (gv : GenericValue) (gvp : GenericValue) (md : metadata) (Mem' : mem)
+  (H : SBopsem.get_reg_metadata TD gl rm vp = ret md)
+  (H0 : getOperandValue TD v lc gl = ret gv)
+  (H1 : getOperandValue TD vp lc gl = ret gvp)
+  (H2 : assert_mptr TD t gvp md)
+  (H3 : mstore TD Mem0 gvp t gv align0 = ret Mem')
+  (H4 : isPointerTypB t = false),
+   exists St' : LLVMopsem.State,
+     exists mi' : meminj,
+       LLVMopsem.dsop_star St St' trace_nil /\
+       sbState_simulates_State mi' mgb
+         {|
+         CurSystem := S;
+         CurTargetData := TD;
+         CurProducts := Ps;
+         ECS := {|
+                CurFunction := F;
+                CurBB := B;
+                CurCmds := cs;
+                Terminator := tmn;
+                Locals := lc;
+                Rmap := rm;
+                Allocas := als |} :: EC;
+         Globals := gl;
+         FunTable := fs;
+         Mem := Mem';
+         Mmap := MM |} St' /\ inject_incr mi mi'.
+Proof.
+  intros.
+  destruct_ctx_other.
+  simpl in Hfresh. destruct Hfresh as [Hnotin Hfresh].
+  apply trans_cmds_inv in Htcmds.
+  destruct Htcmds as [ex_ids5 [cs1' [cs2' [Htcmd [Htcmds Heq]]]]]; subst.
+  simpl in Htcmd. 
+  remember (get_reg_metadata rm2 vp) as R.
+  destruct R as [[bv ev]|]; try solve [inversion Htcmd].
+  remember (mk_tmp ex_ids3) as R1. 
+  destruct R1 as [ptmp ex_ids3'].
+  remember (isPointerTypB t) as R4.
+  destruct R4; try solve [inv H4].
+  inv Htcmd.
+  assert (J:=H2).
+  unfold SBopsem.assert_mptr in J.
+  destruct md as [md_base md_bound].
+  remember (GV2ptr (los,nts) (getPointerSize (los,nts)) gvp) as R.
+  destruct R; try solve [inversion J].
+  destruct v0; try solve [inversion J].
+  remember (GV2ptr (los,nts) (getPointerSize (los,nts)) md_base) as R1.
+  destruct R1; try solve [inversion J].
+  destruct v0; try solve [inversion J].
+  remember (GV2ptr (los,nts) (getPointerSize (los,nts)) md_bound) as R2.
+  destruct R2; try solve [inversion J].
+  destruct v0; try solve [inversion J].
+  remember (getTypeAllocSize (los,nts) t) as R3.
+  destruct R3; try solve [inversion J].
+  eapply simulation__getOperandValue in H0; eauto.
+  destruct H0 as [gv2 [H00 H01]].            
+  eapply simulation__getOperandValue in H1; eauto.
+  destruct H1 as [gvp2 [H10 H11]].            
+  unfold SBopsem.get_reg_metadata in H.
+  assert (Hmstore:=H3).
+  eapply simulation__mstore in H3; eauto.
+  destruct H3 as [Mem2' [H31 [H33 H32]]].
+  assert (J':=Hrsim).
+  destruct J' as [Hrsim1 Hrsim2].
+  assert (HeqR8':=H).
+  apply Hrsim2 in HeqR8'.      
+  destruct HeqR8' as [bv2 [ev2 [bgv2 [egv2 [J1 [J2 [J3 [J4 J5]]]]]]]].
+  rewrite <- HeqR in J1. inv J1.
+  exists (LLVMopsem.mkState S2 (los, nts) Ps2
+          ((LLVMopsem.mkEC (fdef_intro fh2 bs2) B2
+            (cs2' ++ cs23) tmn2 
+              (updateAddAL GenericValue lc2 ptmp gvp2)
+             als2):: 
+            ECs2) gl2 fs2 Mem2').
+  exists mi.
+  split.
+  SSCase "opsem".
+    simpl.
+    rewrite <- (@trace_app_nil__eq__trace trace_nil).
+    apply LLVMopsem.dsop_star_cons with (state2:=
+      (LLVMopsem.mkState S2 (los, nts) Ps2
+          ((LLVMopsem.mkEC (fdef_intro fh2 bs2) B2
+              (insn_call fake_id true attrs assert_typ assert_fn
+                ((p8, bv2)::(p8, ev2)::(p8, value_id ptmp)::(i32, type_size t):: 
+                   (i32, vint1) :: nil):: 
+               insn_store sid t v vp align0 :: 
+               cs2' ++ cs23) tmn2 
+              (updateAddAL GenericValue lc2 ptmp gvp2)
+             als2):: 
+            ECs2) gl2 fs2 M2)).
+      apply LLVMopsem.dsCast; auto.
+        unfold CAST. simpl. simpl in H10.
+        rewrite H10. auto.
+
+    rewrite <- (@trace_app_nil__eq__trace trace_nil).
+    apply LLVMopsem.dsop_star_cons with (state2:=
+      (LLVMopsem.mkState S2 (los, nts) Ps2
+          ((LLVMopsem.mkEC (fdef_intro fh2 bs2) B2
+              (insn_store sid t v vp align0 :: 
+               cs2' ++ cs23) tmn2 
+              (updateAddAL GenericValue lc2 ptmp gvp2)
+             als2):: 
+            ECs2) gl2 fs2 M2)).
+       clear - H00 J2 J3 J4 J5 J H10 H11 HeqR0 HeqR2 HeqR3 HeqR5.
+       eapply assert_mptr_fn__ok with (b:=b)(b0:=b0)(b1:=b1); eauto.
+
+    rewrite <- (@trace_app_nil__eq__trace trace_nil).
+    apply LLVMopsem.dsop_star_cons with (state2:=
+      (LLVMopsem.mkState S2 (los, nts) Ps2
+          ((LLVMopsem.mkEC (fdef_intro fh2 bs2) B2
+              (cs2' ++ cs23) tmn2 
+              (updateAddAL GenericValue lc2 ptmp gvp2)
+             als2):: 
+            ECs2) gl2 fs2 Mem2')); auto.
+      apply LLVMopsem.dsStore with (mp2:=gvp2)(gv1:=gv2); auto.
+        clear - Hnotin HeqR1 HeqR2 HeqR3 H00.
+        destruct Hnotin as [Hnotin1 [_ [Hnotin2 _]]].
+        unfold getCmdIDs in *. simpl in *.
+        rewrite <- getOperandValue_eq_fresh_id; auto.
+          eapply get_reg_metadata_fresh' with (rm2:=rm2); eauto; try fsetdec.
+
+        clear - Hnotin HeqR1 HeqR2 HeqR3 H10.
+        destruct Hnotin as [Hnotin1 [_ [Hnotin2 _]]].
+        unfold getCmdIDs in *. simpl in *.
+        rewrite <- getOperandValue_eq_fresh_id; auto.
+          eapply get_reg_metadata_fresh' with (rm2:=rm2); eauto; try fsetdec.
+
+  split; auto.
+  split; auto.
+  split; auto.
+  split; auto.
+  split; auto.
+  split; auto.
+  split; auto.
+  split; auto.
+  split; auto.
+  split; auto.
+  split; auto.
+  split; auto.
+  split; auto.
+  split; auto.
+  split.
+    eapply cmds_at_block_tail_next; eauto.
+  split.
+    destruct Heqb2 as [l2 [ps2 [cs21 Heqb2]]]; subst.
+    exists l2. exists ps2. exists (cs21 ++
+                  (insn_cast ptmp castop_bitcast (typ_pointer t) vp p8
+                    :: insn_call fake_id true attrs assert_typ assert_fn
+                         ((p8, bv2)
+                          :: (p8, ev2)
+                             :: (p8, value_id ptmp)
+                                :: (i32, type_size t) :: (i32, vint1) :: nil)
+                       :: insn_store sid t v vp align0 :: nil)).
+    simpl_env. auto.
+  exists ex_ids. exists rm2.
+  exists ex_ids5. exists ex_ids4. exists cs2'. exists cs23.
+  split; auto.
+  split.
+    eapply reg_simulation__updateAddAL_tmp; eauto.
+    split; auto.
+      clear - Hinc HeqR1. eapply mk_tmp_inc; eauto.
+    split; auto.
+      clear - Hinc HeqR1 Hfresh. eapply wf_freshs__mk_tmp; eauto.
+  split; auto.
+  split; auto.
+  split; auto.
+  split; auto.
+  SSCase "wfmi".
+    clear - H33 H31 Hmstore Hwfmi.
+    inversion H33.
+    unfold mstore in Hmstore.
+    destruct (GV2ptr (los,nts) (getPointerSize (los,nts)) gvp); 
+      try solve [inversion Hmstore].
+    destruct v; try solve [inversion Hmstore].
+    destruct (typ2memory_chunk t); try solve [inversion Hmstore].
+    destruct (GV2val (los,nts) gv); try solve [inversion Hmstore].
+    erewrite <- Mem.nextblock_store with (m1:=Mem0) in Hmap1; eauto.
+    split; auto.
+    SSSCase "mi_bounds".
+      intros b1 b2 delta J.
+      erewrite Mem.bounds_store with (m1:=Mem0); eauto.
+Qed.
+
+Lemma SBpass_is_correct__dsStore_ptr : forall (mi : meminj) (mgb : Values.block)
+  (St : LLVMopsem.State) (S : system) (TD : TargetData) (Ps : list product)
+  (F : fdef) (B : block) (lc : GVMap) (rm : rmetadata) (gl : GVMap) (fs : GVMap)
+  (sid : id) (t : typ) (align0 : align) (v : value) (vp : value) 
+  (EC : list ExecutionContext) (cs : list cmd) (tmn : terminator) (Mem0 : mem)
+  (MM : mmetadata) (als : list mblock) 
+  (Hsim : sbState_simulates_State mi mgb
+           {|
+           CurSystem := S;
+           CurTargetData := TD;
+           CurProducts := Ps;
+           ECS := {|
+                  CurFunction := F;
+                  CurBB := B;
+                  CurCmds := insn_store sid t v vp align0 :: cs;
+                  Terminator := tmn;
+                  Locals := lc;
+                  Rmap := rm;
+                  Allocas := als |} :: EC;
+           Globals := gl;
+           FunTable := fs;
+           Mem := Mem0;
+           Mmap := MM |} St)
+  (gv : GenericValue) (gvp : GenericValue) (md : metadata)
+  (md' : metadata) (Mem' : mem) (MM' : mmetadata)
+  (H : SBopsem.get_reg_metadata TD gl rm vp = ret md)
+  (H0 : getOperandValue TD v lc gl = ret gv)
+  (H1 : getOperandValue TD vp lc gl = ret gvp)
+  (H2 : assert_mptr TD t gvp md)
+  (H3 : mstore TD Mem0 gvp t gv align0 = ret Mem')
+  (H4 : isPointerTypB t = true)
+  (H5 : SBopsem.get_reg_metadata TD gl rm v = ret md')
+  (H6 : set_mem_metadata TD MM gvp md' = MM'),
+   exists St' : LLVMopsem.State,
+     exists mi' : meminj,
+       LLVMopsem.dsop_star St St' trace_nil /\
+       sbState_simulates_State mi' mgb
+         {|
+         CurSystem := S;
+         CurTargetData := TD;
+         CurProducts := Ps;
+         ECS := {|
+                CurFunction := F;
+                CurBB := B;
+                CurCmds := cs;
+                Terminator := tmn;
+                Locals := lc;
+                Rmap := rm;
+                Allocas := als |} :: EC;
+         Globals := gl;
+         FunTable := fs;
+         Mem := Mem';
+         Mmap := MM' |} St' /\ inject_incr mi mi'.
+Proof.
+  intros.
+  destruct_ctx_other.
+  simpl in Hfresh. destruct Hfresh as [Hnotin Hfresh].
+  apply trans_cmds_inv in Htcmds.
+  destruct Htcmds as [ex_ids5 [cs1' [cs2' [Htcmd [Htcmds Heq]]]]]; subst.
+  simpl in Htcmd. 
+  remember (get_reg_metadata rm2 vp) as R.
+  destruct R as [[bv ev]|]; try solve [inversion Htcmd].
+  remember (mk_tmp ex_ids3) as R1. 
+  destruct R1 as [ptmp ex_ids3'].
+  remember (isPointerTypB t) as R4.
+  destruct R4; try solve [inv H4].
+  remember (get_reg_metadata rm2 v) as R5.
+  destruct R5 as [[bv0 ev0]|]; inv Htcmd.
+  assert (J:=H2).
+  unfold SBopsem.assert_mptr in J.
+  destruct md as [md_base md_bound].
+  remember (GV2ptr (los,nts) (getPointerSize (los,nts)) gvp) as R.
+  destruct R; try solve [inversion J].
+  destruct v0; try solve [inversion J].
+  remember (GV2ptr (los,nts) (getPointerSize (los,nts)) md_base) as R1.
+  destruct R1; try solve [inversion J].
+  destruct v0; try solve [inversion J].
+  remember (GV2ptr (los,nts) (getPointerSize (los,nts)) md_bound) as R2.
+  destruct R2; try solve [inversion J].
+  destruct v0; try solve [inversion J].
+  remember (getTypeAllocSize (los,nts) t) as R3.
+  destruct R3; try solve [inversion J].
+  eapply simulation__getOperandValue in H0; eauto.
+  destruct H0 as [gv2 [H00 H01]].            
+  eapply simulation__getOperandValue in H1; eauto.
+  destruct H1 as [gvp2 [H10 H11]].            
+  unfold SBopsem.get_reg_metadata in H.
+  assert (H3':=H3).
+  eapply simulation__mstore in H3'; eauto.
+  destruct H3' as [Mem2' [H31 [H33 H32]]].
+  assert (J':=Hrsim).
+  destruct J' as [Hrsim1 Hrsim2].
+
+  destruct md' as [md_base' md_bound'].
+  assert (HeqR9':=H).
+  apply Hrsim2 in HeqR9'.      
+  destruct HeqR9' as [bv2 [ev2 [bgv2 [egv2 [J1 [J2 [J3 [J4 J5]]]]]]]].
+  assert (H5':=H5).      
+  apply Hrsim2 in H5'.
+  destruct H5' as [bv2' [ev2' [bgv2' [egv2' [J1' [J2' [J3' [J4' J5']]]]]]]].
+  simpl in HeqR5.
+  rewrite J1' in HeqR5.
+  inv HeqR5.
+  rewrite <- HeqR in J1. inv J1.
+
+  assert (exists Mem2'',
+    LLVMopsem.dsInsn
+      (LLVMopsem.mkState S2 (los, nts) Ps2
+          ((LLVMopsem.mkEC (fdef_intro fh2 bs2) B2
+              (insn_call fake_id true attrs smmd_typ smmd_fn
+                ((p8, value_id ptmp) :: (p8, bv2') :: (p8, ev2') :: (p8, vnullp8)
+                    :: (i32, vint1) :: (i32, vint1) :: nil):: 
+               cs2' ++ cs23) tmn2 
+              (updateAddAL GenericValue lc2 ptmp gvp2)
+             als2):: 
+            ECs2) gl2 fs2 Mem2')
+      (LLVMopsem.mkState S2 (los, nts) Ps2
+          ((LLVMopsem.mkEC (fdef_intro fh2 bs2) B2
+              (cs2' ++ cs23) tmn2 
+              (updateAddAL GenericValue lc2 ptmp gvp2)
+             als2):: 
+            ECs2) gl2 fs2 Mem2'') trace_nil /\
+      mem_simulation mi (los,nts) mgb
+        (SBopsem.set_mem_metadata (los,nts) MM gvp 
+          (SBopsem.mkMD md_base' md_bound')) 
+        Mem' Mem2'') as W.
+    assert (exists b : Values.block, exists ofs : int32, exists cm,
+      gvp = (Vptr b ofs,cm)::nil) as EQ.
+      clear - H11 H31 H3.
+      eapply mstore_inversion; eauto.
+    destruct EQ as [b2 [ofs2 [cm EQ]]]. subst.
+
+    eapply simulation__set_mmetadata_fn with (pgv':=gvp2)(bgv':=bgv2')
+      (egv':=egv2')(rm:=rm)(v:=v); simpl; eauto.
+      clear - HeqR1 HeqR2 HeqR3.
+      rewrite lookupAL_updateAddAL_eq; auto.
+
+      clear - J2' H31 J1' Hnotin HeqR1 HeqR2 HeqR3.
+      rewrite <- getOperandValue_eq_fresh_id; eauto.
+        eapply get_reg_metadata__fresh with (rm2:=rm2)
+          (c:=insn_store sid t v vp align0) in J1'; 
+          eauto; try fsetdec. destruct J1'; auto.
+
+      clear - J3' H31 J1' Hnotin HeqR1 HeqR2 HeqR3.
+      rewrite <- getOperandValue_eq_fresh_id; eauto.
+        eapply get_reg_metadata__fresh with (rm2:=rm2)
+          (c:=insn_store sid t v vp align0) in J1'; 
+          eauto; try fsetdec. destruct J1'; auto.
+
+  destruct W as [Mem2'' [W1 W2]].
+
+  exists (LLVMopsem.mkState S2 (los, nts) Ps2
+          ((LLVMopsem.mkEC (fdef_intro fh2 bs2) B2
+            (cs2' ++ cs23) tmn2 
+              (updateAddAL GenericValue lc2 ptmp gvp2)
+             als2):: 
+            ECs2) gl2 fs2 Mem2'').
+  exists mi.
+  split.
+  SSCase "opsem".
+    simpl.
+    rewrite <- (@trace_app_nil__eq__trace trace_nil).
+    apply LLVMopsem.dsop_star_cons with (state2:=
+      (LLVMopsem.mkState S2 (los, nts) Ps2
+          ((LLVMopsem.mkEC (fdef_intro fh2 bs2) B2
+              (insn_call fake_id true attrs assert_typ assert_fn
+                ((p8, bv2)::(p8, ev2)::(p8, value_id ptmp)::(i32, type_size t):: 
+                   (i32, vint1) :: nil):: 
+               insn_store sid t v vp align0 :: 
+               insn_call fake_id true attrs smmd_typ smmd_fn
+                ((p8, value_id ptmp) :: (p8, bv2') :: (p8, ev2') :: (p8, vnullp8)
+                    :: (i32, vint1) :: (i32, vint1) :: nil):: 
+              cs2' ++ cs23) tmn2 
+              (updateAddAL GenericValue lc2 ptmp gvp2)
+             als2):: 
+            ECs2) gl2 fs2 M2)).
+      apply LLVMopsem.dsCast; auto.
+        unfold CAST. simpl. simpl in H10.
+        rewrite H10. auto.
+
+    rewrite <- (@trace_app_nil__eq__trace trace_nil).
+    apply LLVMopsem.dsop_star_cons with (state2:=
+      (LLVMopsem.mkState S2 (los, nts) Ps2
+          ((LLVMopsem.mkEC (fdef_intro fh2 bs2) B2
+              (insn_store sid t v vp align0 :: 
+               insn_call fake_id true attrs smmd_typ smmd_fn
+                ((p8, value_id ptmp) :: (p8, bv2') :: (p8, ev2') :: (p8, vnullp8)
+                    :: (i32, vint1) :: (i32, vint1) :: nil):: 
+               cs2' ++ cs23) tmn2 
+              (updateAddAL GenericValue lc2 ptmp gvp2)
+             als2):: 
+            ECs2) gl2 fs2 M2)).
+       clear - H00 J2 J3 J4 J5 J H10 H11 HeqR0 HeqR2 HeqR3 HeqR6.
+       eapply assert_mptr_fn__ok with (b:=b)(b0:=b0)(b1:=b1); eauto.
+
+    rewrite <- (@trace_app_nil__eq__trace trace_nil).
+    apply LLVMopsem.dsop_star_cons with (state2:=
+      (LLVMopsem.mkState S2 (los, nts) Ps2
+          ((LLVMopsem.mkEC (fdef_intro fh2 bs2) B2
+              (insn_call fake_id true attrs smmd_typ smmd_fn
+                ((p8, value_id ptmp) :: (p8, bv2') :: (p8, ev2') :: (p8, vnullp8)
+                    :: (i32, vint1) :: (i32, vint1) :: nil):: 
+               cs2' ++ cs23) tmn2 
+              (updateAddAL GenericValue lc2 ptmp gvp2)
+             als2):: 
+            ECs2) gl2 fs2 Mem2')); auto.
+      apply LLVMopsem.dsStore with (mp2:=gvp2)(gv1:=gv2); auto.
+        clear - Hnotin HeqR1 HeqR2 HeqR3 H00.
+        destruct Hnotin as [Hnotin1 [_ [Hnotin2 _]]].
+        unfold getCmdIDs in *. simpl in *.
+        rewrite <- getOperandValue_eq_fresh_id; auto.
+          eapply get_reg_metadata_fresh' with (rm2:=rm2); eauto; try fsetdec.
+
+        clear - Hnotin HeqR1 HeqR2 HeqR3 H10.
+        destruct Hnotin as [Hnotin1 [_ [Hnotin2 _]]].
+        unfold getCmdIDs in *. simpl in *.
+        rewrite <- getOperandValue_eq_fresh_id; auto.
+          eapply get_reg_metadata_fresh' with (rm2:=rm2); eauto; try fsetdec.
+
+    rewrite <- (@trace_app_nil__eq__trace trace_nil).
+    eapply LLVMopsem.dsop_star_cons; eauto.
+
+  split; auto.
+  split; auto.
+  split; auto.
+  split; auto.
+  split; auto.
+  split; auto.
+  split; auto.
+  split; auto.
+  split; auto.
+  split; auto.
+  split; auto.
+  split; auto.
+  split; auto.
+  split; auto.
+  split.
+    eapply cmds_at_block_tail_next; eauto.
+  split.
+    destruct Heqb2 as [l2 [ps2 [cs21 Heqb2]]]; subst.
+    exists l2. exists ps2. exists (cs21 ++
+                  (insn_cast ptmp castop_bitcast (typ_pointer t) vp p8
+                    :: insn_call fake_id true attrs assert_typ assert_fn
+                         ((p8, bv2)
+                          :: (p8, ev2)
+                             :: (p8, value_id ptmp)
+                                :: (i32, type_size t) :: (i32, vint1) :: nil)
+                       :: insn_store sid t v vp align0 :: 
+                   insn_call fake_id true attrs smmd_typ smmd_fn
+                      ((p8, value_id ptmp) :: (p8, bv2') :: (p8, ev2') :: 
+                      (p8, vnullp8) :: (i32, vint1) :: (i32, vint1) :: nil)::   
+                   nil)).
+    simpl_env. auto.
+  exists ex_ids. exists rm2.
+  exists ex_ids5. exists ex_ids4. exists cs2'. exists cs23.
+  split; auto.
+  split.
+    eapply reg_simulation__updateAddAL_tmp; eauto.
+    split; auto.
+      clear - Hinc HeqR1. eapply mk_tmp_inc; eauto.
+    split; auto.
+      clear - Hinc HeqR1 Hfresh. eapply wf_freshs__mk_tmp; eauto.
+  split; auto.
+  split; auto.
+  split; auto.
+  split; auto.
+  SSCase "wfmi".
+    clear - H33 H31 H3 Hwfmi W1.
+    inversion H33.
+    unfold mstore in H3.
+    destruct (GV2ptr (los,nts) (getPointerSize (los,nts)) gvp); 
+      try solve [inversion H3].
+    destruct v; try solve [inversion H3].
+    destruct (typ2memory_chunk t); try solve [inversion H3].
+    destruct (GV2val (los,nts) gv); try solve [inversion H3].
+    erewrite <- Mem.nextblock_store with (m1:=Mem0) in Hmap1; eauto.
+    apply set_mmetadata_fn__prop in W1.
+    destruct W1 as [W1 [W2 W3]].
+    split; auto.
+    SSSCase "Hmap4".
+      intros b1 b2 delta2 J.
+      apply Hmap2 in J.
+      eauto with zarith.
+    SSSCase "mappedblocks0".
+      intros b1 b2 delta J.
+      apply mi_mappedblocks in J.
+      eauto.
+    SSSCase "bounds0".
+      intros b1 b2 delta J.
+      apply mi_bounds in J.
+      rewrite <- W3.
+      erewrite Mem.bounds_store with (m1:=Mem0); eauto.
+Qed.
+
+
+Lemma SBpass_is_correct__dsAlloca : forall 
+  (mi : meminj) (mgb : Values.block) (St : LLVMopsem.State) (S : system)
+  (TD : TargetData) (Ps : list product) (F : fdef) (B : block) (lc : GVMap)
+  (rm : AssocList metadata) (gl : GVMap) (fs : GVMap) (id0 : atom) (t : typ)  
+  (v : value) (align0 : align) (EC : list ExecutionContext) (cs : list cmd)
+  (tmn : terminator) (Mem0 : mem) (MM : mmetadata) (als : list mblock)
+  (Hsim : sbState_simulates_State mi mgb
+           {|
+           CurSystem := S;
+           CurTargetData := TD;
+           CurProducts := Ps;
+           ECS := {|
+                  CurFunction := F;
+                  CurBB := B;
+                  CurCmds := insn_alloca id0 t v align0 :: cs;
+                  Terminator := tmn;
+                  Locals := lc;
+                  Rmap := rm;
+                  Allocas := als |} :: EC;
+           Globals := gl;
+           FunTable := fs;
+           Mem := Mem0;
+           Mmap := MM |} St)
+  (gn : GenericValue) (Mem' : mem) (tsz : sz) (mb : mblock) (lc' : GVMap)
+  (rm' : rmetadata) (n : Z) (H : getTypeAllocSize TD t = ret tsz)
+  (H0 : getOperandValue TD v lc gl = ret gn) 
+  (H1 : malloc TD Mem0 tsz gn align0 = ret (Mem', mb))
+  (H2 : GV2int TD Size.ThirtyTwo gn = ret n)
+  (H3 : prop_reg_metadata lc rm id0 (blk2GV TD mb)
+         {| md_base := base2GV TD mb; md_bound := bound2GV TD mb tsz n |} =
+       (lc', rm')),
+   exists St' : LLVMopsem.State,
+     exists mi' : meminj,
+       LLVMopsem.dsop_star St St' trace_nil /\
+       sbState_simulates_State mi' mgb
+         {|
+         CurSystem := S;
+         CurTargetData := TD;
+         CurProducts := Ps;
+         ECS := {|
+                CurFunction := F;
+                CurBB := B;
+                CurCmds := cs;
+                Terminator := tmn;
+                Locals := lc';
+                Rmap := rm';
+                Allocas := mb :: als |} :: EC;
+         Globals := gl;
+         FunTable := fs;
+         Mem := Mem';
+         Mmap := MM |} St' /\ inject_incr mi mi'.
+Proof.
+  intros.
+  destruct_ctx_other.
+  simpl in Hfresh. destruct Hfresh as [Hnotin Hfresh].
+  apply trans_cmds_inv in Htcmds.
+  destruct Htcmds as [ex_ids5 [cs1' [cs2' [Htcmd [Htcmds Heq]]]]]; subst.
+  simpl in Htcmd.
+  remember (lookupAL (id * id) rm2 id0) as R1.
+  destruct R1 as [[bid eid]|]; try solve [inversion Htcmd].
+  remember (mk_tmp ex_ids3) as R2.
+  destruct R2 as [tmp ex_ids6].
+  inv Htcmd.
+  invert_prop_reg_metadata.
+  assert (Hmalloc:=H1).
+  apply mem_simulation__malloc with (MM:=MM)(mgb:=mgb)(Mem2:=M2)(mi:=mi) in H1;
+    auto.
+  destruct H1 as [mi' [Mem2' [mb' [H11 [H16 [H12 [H13 [H14 H15]]]]]]]].
+  simpl.
+  exists (LLVMopsem.mkState S2 (los, nts) Ps2
+          ((LLVMopsem.mkEC (fdef_intro fh2 bs2) B2
+            (cs2' ++ cs23) tmn2 
+                (updateAddAL _ 
+                  (updateAddAL _ 
+                    (updateAddAL _ 
+                      (updateAddAL GenericValue lc2 id0 (blk2GV (los, nts) mb'))
+                      tmp (SBopsem.bound2GV (los, nts) mb' tsz n))
+                    bid (SBopsem.base2GV (los, nts) mb'))
+                  eid (SBopsem.bound2GV (los, nts) mb' tsz n))
+             (mb'::als2)):: 
+            ECs2) gl2 fs2 Mem2').
+  exists mi'.
+  split.
+  SCase "opsem".
+    rewrite <- (@trace_app_nil__eq__trace trace_nil).
+    apply LLVMopsem.dsop_star_cons with (state2:=
+        LLVMopsem.mkState S2 (los, nts) Ps2
+          ((LLVMopsem.mkEC (fdef_intro fh2 bs2) B2
+             (insn_gep tmp false t (value_id id0) 
+                (Cons_list_value v Nil_list_value):: 
+              insn_cast bid castop_bitcast (typ_pointer t)(value_id id0) p8 :: 
+              insn_cast eid castop_bitcast (typ_pointer t)(value_id tmp) p8 :: 
+              cs2' ++ cs23)
+             tmn2 
+             (updateAddAL GenericValue lc2 id0 (blk2GV (los, nts) mb'))
+             (mb'::als2)):: 
+            ECs2) gl2 fs2 Mem2'); auto.
+      eapply simulation__getOperandValue with (mi:=mi)(Mem2:=M2) in H0; eauto.
+      destruct H0 as [gn' [H00 H01]].
+      unfold malloc in H11.
+      erewrite simulation__eq__GV2int in H11; eauto.
+
+    rewrite <- (@trace_app_nil__eq__trace trace_nil).
+    apply LLVMopsem.dsop_star_cons with (state2:=
+        LLVMopsem.mkState S2 (los, nts) Ps2
+          ((LLVMopsem.mkEC (fdef_intro fh2 bs2) B2
+             (insn_cast bid castop_bitcast (typ_pointer t)(value_id id0) p8 :: 
+              insn_cast eid castop_bitcast (typ_pointer t)(value_id tmp) p8 :: 
+              cs2' ++ cs23)
+             tmn2 
+             (updateAddAL _
+               (updateAddAL GenericValue lc2 id0 (blk2GV (los,nts) mb'))
+               tmp (SBopsem.bound2GV (los,nts) mb' tsz n))
+             (mb'::als2)):: 
+            ECs2) gl2 fs2 Mem2'); auto.
+      assert (exists gn', getOperandValue (los,nts) v lc2 gl2 = ret gn' /\
+          GV2int (los,nts) Size.ThirtyTwo gn = 
+          GV2int (los,nts) Size.ThirtyTwo gn') as H4.
+        eapply simulation__getOperandValue with (Mem2:=M2) in H0; eauto.
+        destruct H0 as [gv' [H00 H01]].
+        exists gv'. split; auto.
+          rewrite simulation__eq__GV2int with (mi:=mi)(gn':=gv'); eauto.
+      destruct H4 as [gn' [H41 H42]].
+      apply LLVMopsem.dsGEP with (mp:=blk2GV (los,nts) mb')(vidxs:=[gn']); auto.
+        simpl.
+        rewrite lookupAL_updateAddAL_eq; auto.
+
+        simpl.
+        assert(getOperandValue (los,nts) v
+          (updateAddAL _ lc2 id0 (blk2GV (los,nts) mb')) gl2 = 
+          getOperandValue (los,nts) v lc2 gl2) as EQ'.
+          clear - Hnotin HeqR1. 
+          destruct Hnotin as [Hnotin1 [Hnotin2 _ ]]. simpl in Hnotin2.
+
+          rewrite <- getOperandValue_eq_fresh_id; auto.
+            unfold getCmdIDs in Hnotin1. simpl in Hnotin1.
+            eapply notin_codom__neq' in HeqR1; eauto.
+              destruct v; simpl in *; fsetdec.
+
+        rewrite EQ'. clear EQ'.
+        rewrite H41. auto.
+
+        unfold SBopsem.bound2GV, GEP, blk2GV, GV2ptr, ptr2GV, val2GV.
+        simpl.
+        rewrite <- H42. rewrite H2.
+        unfold Constant.typ2utyp.
+        assert (exists ut, 
+          Constant.typ2utyp_aux (Constant.subst_nts_by_nts nts nts) 
+            (typ_array 0%nat t) = Some (typ_array 0%nat ut) /\
+          getTypeAllocSize (los, nts) ut = getTypeAllocSize (los, nts) t) as EQ1.
+          destruct Heqb1 as [l1 [ps1 [cs11 Heqb1]]]; subst.
+          eapply wf_system__wf_cmd with (c:=insn_alloca id0 t v align0) in HBinF;
+            eauto.
+            inv HBinF. inv H21. 
+            (* ssa_static should check this typ is Constant.unifiable_typ
+               like wf_const_gid *)
+            admit.
+            apply in_or_app. simpl. auto.
+        destruct EQ1 as [ut [EQ1 EQ2]].
+        rewrite EQ1. simpl.
+        rewrite EQ2. rewrite H. simpl.
+        rewrite Int.add_commut.
+        rewrite Int.add_zero. auto.
+
+    rewrite <- (@trace_app_nil__eq__trace trace_nil).
+    apply LLVMopsem.dsop_star_cons with (state2:=
+        LLVMopsem.mkState S2 (los, nts) Ps2
+          ((LLVMopsem.mkEC (fdef_intro fh2 bs2) B2
+             (insn_cast eid castop_bitcast (typ_pointer t)(value_id tmp) p8 :: 
+              cs2' ++ cs23)
+             tmn2 
+             (updateAddAL _
+               (updateAddAL _
+                 (updateAddAL GenericValue lc2 id0 (blk2GV (los,nts) mb'))
+                 tmp (SBopsem.bound2GV (los,nts) mb' tsz n))
+               bid (SBopsem.base2GV (los,nts) mb'))               
+             (mb'::als2)):: 
+            ECs2) gl2 fs2 Mem2'); auto.
+      apply LLVMopsem.dsCast; auto.
+        unfold CAST. simpl.
+        rewrite <- lookupAL_updateAddAL_neq.
+          rewrite lookupAL_updateAddAL_eq.
+          auto.
+
+          clear - Hnotin HeqR1 HeqR2.
+          destruct Hnotin as [Hnotin1 [_ [Hnotin2 _]]]. 
+          unfold getCmdIDs in *. simpl in *.
+          eapply tmp_is_fresh; eauto. fsetdec.
+
+    rewrite <- (@trace_app_nil__eq__trace trace_nil).
+    apply LLVMopsem.dsop_star_cons with (state2:=
+       (LLVMopsem.mkState S2 (los, nts) Ps2
+          ((LLVMopsem.mkEC (fdef_intro fh2 bs2) B2
+            (cs2' ++ cs23) tmn2 
+                (updateAddAL _ 
+                  (updateAddAL _ 
+                    (updateAddAL _ 
+                      (updateAddAL GenericValue lc2 id0 (blk2GV (los, nts) mb'))
+                      tmp (SBopsem.bound2GV (los, nts) mb' tsz n))
+                    bid (SBopsem.base2GV (los, nts) mb'))                    
+                  eid (SBopsem.bound2GV (los, nts) mb' tsz n))
+             (mb'::als2)):: 
+            ECs2) gl2 fs2 Mem2')); auto.
+      apply LLVMopsem.dsCast; auto.
+        unfold CAST. simpl.
+        rewrite <- lookupAL_updateAddAL_neq.
+          rewrite lookupAL_updateAddAL_eq; auto.
+
+          destruct Hnotin as [Hnotin1 [Hnotin2 [Hnotin3 Hnotin4]]]. 
+          unfold getCmdIDs in *.
+          eapply tmp_is_fresh' with (tmp:=tmp) in HeqR1; eauto. 
+            destruct HeqR1; auto.
+            clear - Hnotin3. fsetdec.
+
+  split; auto.
+  split; auto.
+  split; auto.
+  split; auto.
+  split.
+  split.
+  split; auto.          
+  split; auto.          
+  split; auto.
+  split; auto.
+  split; auto.
+  split; auto.
+  split; auto.
+  split; auto.
+    split; eauto using inject_incr__preserves__als_simulation.
+  split; auto.          
+  split; auto.          
+    eapply cmds_at_block_tail_next; eauto.
+  split.
+    destruct Heqb2 as [l2 [ps2 [cs21 Heqb2]]]; subst.
+    exists l2. exists ps2. exists (cs21 ++
+                  (insn_alloca id0 t v align0
+                    :: insn_gep tmp false t (value_id id0)
+                         (Cons_list_value v Nil_list_value)
+                       :: insn_cast bid castop_bitcast 
+                            (typ_pointer t) (value_id id0) p8
+                          :: insn_cast eid castop_bitcast 
+                               (typ_pointer t) (value_id tmp) p8 :: nil)).
+    simpl_env. auto.
+  exists ex_ids. exists rm2.
+  exists ex_ids5. exists ex_ids4. exists cs2'. exists cs23.
+  split; auto.
+  split.
+  SCase "rsim".
+    eapply reg_simulation__updateAddAL_md; eauto.
+      eapply reg_simulation__updateAddAL_tmp; eauto.
+      eapply reg_simulation__updateAddAL_lc; eauto.
+        eapply inject_incr__preserves__reg_simulation; eauto.
+        admit.
+        admit.
+
+      unfold gv_inject, blk2GV, ptr2GV, val2GV.
+      simpl. apply val_cons_inject; eauto.
+
+      unfold gv_inject, SBopsem.base2GV, blk2GV, ptr2GV, val2GV.
+      simpl. clear - H14.
+      apply val_cons_inject; eauto.
+
+      unfold gv_inject, SBopsem.base2GV, blk2GV, ptr2GV, val2GV.
+      simpl. clear - H14.
+        apply val_cons_inject; eauto.
+          eapply val_inject_ptr; eauto.
+            rewrite Int.add_zero. auto.
+
+    split; auto.
+      clear - Hinc HeqR2. eapply mk_tmp_inc; eauto.
+    split; auto.
+      clear - Hinc HeqR2 Hfresh. eapply wf_freshs__mk_tmp; eauto.
+      
+      clear - HsimECs H13. 
+      eapply inject_incr__preserves__sbECs_simulate_ECs_tail; eauto.
+Qed.
+
+Lemma SBpass_is_correct : forall mi mgb sbSt St sbSt' tr,
+  sbState_simulates_State mi mgb sbSt St ->
+  SBopsem.dsInsn sbSt sbSt' tr -> 
+  exists St', exists mi',
+    LLVMopsem.dsop_star St St' tr /\    
+    sbState_simulates_State mi' mgb sbSt' St' /\
+    Values.inject_incr mi mi'.
+Proof.
+  intros mi mgb sbSt St sbSt' tr Hsim Hsbop.
+  (sb_dsInsn_cases (induction Hsbop) Case).
+Case "dsReturn". eapply SBpass_is_correct__dsReturn; eauto.
+Case "dsReturnVoid". eapply SBpass_is_correct__dsReturnVoid; eauto.
+Case "dsBranch". admit.
+Case "dsBranch_uncond". Focus.
+
+Ltac destruct_ctx_br :=
+match goal with
+| [Hsim : sbState_simulates_State _ _
+           {|
+           SBopsem.CurSystem := _;
+           SBopsem.CurTargetData := ?TD;
+           SBopsem.CurProducts := _;
+           SBopsem.ECS := {|
+                          SBopsem.CurFunction := ?F;
+                          SBopsem.CurBB := _;
+                          SBopsem.CurCmds := nil;
+                          SBopsem.Terminator := _;
+                          SBopsem.Locals := _;
+                          SBopsem.Rmap := _;
+                          SBopsem.Allocas := _ |} :: _;
+           SBopsem.Globals := _;
+           SBopsem.FunTable := _;
+           SBopsem.Mem := _;
+           SBopsem.Mmap := _ |} ?St |- _] =>
+  destruct St as [S2 TD2 Ps2 ECs2 gl2 fs2 M2];
+  destruct TD as [los nts];
+  destruct Hsim as [Hwfs [HMinS [Htsym [Heq1 [Htps [HsimECs [Heq2 [Heq3 [Hwfg 
+    [Hwfmi HsimM]]]]]]]]]];
+    subst;
+  destruct ECs2 as [|[F2 B2 cs2 tmn2 lc2 als2] ECs2];
+    try solve [inversion HsimECs];
+  simpl in HsimECs;
+  destruct HsimECs as [HsimEC HsimECs];
+  destruct F as [fh1 bs1];
+  destruct F2 as [fh2 bs2];
+  destruct HsimEC as [HBinF [HFinPs [Htfdef [Heq0 [Hasim [Hnth [Heqb1 [Heqb2 
+    [ex_ids [rm2 [ex_ids3 [ex_ids4 [cs22 [cs23 [Hgenmeta [Hrsim [Hinc [Hfresh 
+    [Htcmds [Httmn Heq2]]]]]]]]]]]]]]]]]]]]; subst
+end.
+
+  destruct_ctx_br.
+  simpl in Hfresh. destruct Hfresh as [Hnotin Hfresh].
+  inv Htcmds. inv Httmn.
+
+Lemma lookup_trans_blocks__trans_block : forall bs1 bs2 ex_ids0 ex_ids ex_ids'
+    l0 b1 rm,
+  uniqBlocks bs1 ->
+  incl ex_ids0 ex_ids ->
+  trans_blocks ex_ids rm bs1 = Some (ex_ids', bs2) ->
+  lookupBlockViaLabelFromBlocks bs1 l0 = Some b1 ->
+  exists ex_ids1, exists ex_ids2, exists b2, exists n,
+    lookupBlockViaLabelFromBlocks bs2 l0 = Some b2 /\
+    trans_block ex_ids1 rm b1 = Some (ex_ids2, b2) /\
+    incl ex_ids0 ex_ids1 /\
+    nth_error bs1 n = Some b1 /\
+    nth_error bs2 n = Some b2.
+Admitted.
+
+     
+admit.
+
+Case "dsBop". eapply SBpass_is_correct__dsBop; eauto.
+admit. admit. admit.
+
+Case "dsMalloc". eapply SBpass_is_correct__dsMalloc; eauto.
+Case "dsFree". eapply SBpass_is_correct__dsFree; eauto.
+Case "dsAlloca". eapply SBpass_is_correct__dsAlloca; eauto.
+
+Case "dsLoad_nptr". eapply SBpass_is_correct__dsLoad_nptr; eauto.
+Case "dsLoad_ptr". eapply SBpass_is_correct__dsLoad_ptr; eauto.
+Case "dsStore_nptr". eapply SBpass_is_correct__dsStore_nptr; eauto.
+Case "dsStore_ptr". eapply SBpass_is_correct__dsStore_ptr; eauto.
+
+Admitted.
 
 (*****************************)
 (*
@@ -611,3 +2742,5 @@ Admitted.
 *** coq-prog-args: ("-emacs-U" "-I" "~/SVN/sol/vol/src/ssa/monads" "-I" "~/SVN/sol/vol/src/ssa/ott" "-I" "~/SVN/sol/vol/src/ssa/compcert" "-I" "~/SVN/sol/theory/metatheory_8.3" "-I" "~/SVN/sol/vol/src/TV") ***
 *** End: ***
  *)
+
+
